Iris Proofmode.

heap_lang/lib/barrier/client.v
@@ -1,6 +1,7 @@
 From iris.heap_lang.lib.barrier Require Import proof.
 From iris.heap_lang Require Import par.
 From iris.program_logic Require Import auth sts saved_prop hoare ownership.
+From iris.heap_lang Require Import proofmode.
 Import uPred.
 
 Definition worker (n : Z) : val :=
@@ -15,63 +16,44 @@ Section client.
   Context {Σ : gFunctors} `{!heapG Σ, !barrierG Σ, !spawnG Σ} (heapN N : namespace).
   Local Notation iProp := (iPropG heap_lang Σ).
 
-  Definition y_inv q y : iProp :=
-    (∃ f : val, y ↦{q} f ★ □ ∀ n : Z, WP f #n {{ λ v, v = #(n + 42) }})%I.
+  Definition y_inv (q : Qp) (l : loc) : iProp :=
+    (∃ f : val, l ↦{q} f ★ □ ∀ n : Z, WP f #n {{ λ v, v = #(n + 42) }})%I.
 
-  Lemma y_inv_split q y :
-    y_inv q y ⊢ (y_inv (q/2) y ★ y_inv (q/2) y).
+  Lemma y_inv_split q l : y_inv q l ⊢ (y_inv (q/2) l ★ y_inv (q/2) l).
   Proof.
-    rewrite /y_inv. apply exist_elim=>f.
-    rewrite -!(exist_intro f). rewrite heap_mapsto_op_split.
-    ecancel [y ↦{_} _; y ↦{_} _]%I. by rewrite [X in X ⊢ _]always_sep_dup.
+    iIntros "Hl"; iDestruct "Hl" as {f} "[[Hl1 Hl2] #Hf]".
+    iSplitL "Hl1"; iExists f; by iSplitL; try iAlways.
   Qed.
 
   Lemma worker_safe q (n : Z) (b y : loc) :
     (heap_ctx heapN ★ recv heapN N b (y_inv q y))
-      ⊢ WP worker n (%b) (%y) {{ λ _, True }}.
+    ⊢ WP worker n (%b) (%y) {{ λ _, True }}.
   Proof.
-    rewrite /worker. wp_lam. wp_let. ewp apply wait_spec.
-    rewrite comm. apply sep_mono_r. apply wand_intro_l.
-    rewrite sep_exist_r. apply exist_elim=>f. wp_seq.
-    (* TODO these parenthesis are rather surprising. *)
-    (ewp apply: (wp_load heapN _ _ q f)); eauto with I.
-    strip_later. (* hu, shouldn't it do that? *)
-    rewrite -assoc. apply sep_mono_r. apply wand_intro_l.
-    rewrite always_elim (forall_elim n) sep_elim_r sep_elim_l.
-    apply wp_mono=>?. eauto with I.
+    iIntros "[#Hh Hrecv]". wp_lam. wp_let.
+    wp_apply wait_spec; iFrame "Hrecv".
+    iIntros "Hy"; iDestruct "Hy" as {f} "[Hy #Hf]".
+    wp_seq. wp_load.
+    iApply wp_wand_r; iSplitR; [iApply "Hf"|by iIntros {v} "_"].
   Qed.
 
-  Lemma client_safe :
-    heapN ⊥ N → heap_ctx heapN ⊢ WP client {{ λ _, True }}.
+  Lemma client_safe : heapN ⊥ N → heap_ctx heapN ⊢ WP client {{ λ _, True }}.
   Proof.
-    intros ?. rewrite /client.
-    (ewp eapply wp_alloc); eauto with I. strip_later. apply forall_intro=>y.
-    apply wand_intro_l. wp_let.
-    ewp eapply (newbarrier_spec heapN N (y_inv 1 y)); last done.
-    rewrite comm. rewrite {1}[heap_ctx _]always_sep_dup -!assoc.
-    apply sep_mono_r. apply forall_intro=>b. apply wand_intro_l. 
-    wp_let. (ewp eapply (wp_par heapN N (λ _, True%I) (λ _, True%I))); eauto.
-    rewrite 2!{1}[heap_ctx _]always_sep_dup !assoc [(_ ★ heap_ctx _)%I]comm.
-    ecancel [heap_ctx _]. sep_split right: []; last first.
-    { do 2 apply forall_intro=>_. apply wand_intro_l.
-      eauto using later_intro with I. }
-    sep_split left: [send heapN _ _ _; heap_ctx _; y ↦ _]%I.
+    iIntros {?} "#Hh"; rewrite /client. wp_alloc y as "Hy". wp_let.
+    wp_apply (newbarrier_spec heapN N (y_inv 1 y)); first done.
+    iFrame "Hh". iIntros {l} "[Hr Hs]". wp_let.
+    iApply (wp_par heapN N (λ _, True%I) (λ _, True%I)); first done.
+    iFrame "Hh". iSplitL "Hy Hs".
     - (* The original thread, the sender. *)
-      (ewp eapply wp_store); eauto with I. strip_later.
-      ecancel [y ↦ _]%I. apply wand_intro_l.
-      wp_seq. rewrite -signal_spec right_id assoc sep_elim_l comm.
-      apply sep_mono_r. rewrite /y_inv -(exist_intro (λ: "z", '"z" + #42)%V).
-      apply sep_intro_True_r; first done. apply: always_intro.
-      apply forall_intro=>n. wp_let. wp_op. by apply const_intro.
+      wp_store. wp_seq. iApply signal_spec; iFrame "Hs"; iSplit; [|done].
+      iExists _; iSplitL; [done|]. iAlways; iIntros {n}. wp_let. by wp_op.
     - (* The two spawned threads, the waiters. *)
-      rewrite recv_mono; last exact: y_inv_split.
-      rewrite (recv_split _ _ ⊤) // pvs_frame_r. apply wp_strip_pvs.
-      (ewp eapply (wp_par heapN N (λ _, True%I) (λ _, True%I))); eauto.
-      do 2 rewrite {1}[heap_ctx _]always_sep_dup.
-      ecancel [heap_ctx _]. rewrite !assoc. sep_split right: []; last first.
-      { do 2 apply forall_intro=>_. apply wand_intro_l.
-        eauto using later_intro with I. }
-      sep_split left: [recv heapN _ _ _; heap_ctx _]%I; by rewrite -worker_safe comm.
+      iSplitL; [|iIntros {_ _} "_"; by iNext].
+      iDestruct recv_weaken "[] Hr" as "Hr".
+      { iIntros "?". by iApply y_inv_split "-". }
+      iPvs recv_split "Hr" as "[H1 H2]"; first done.
+      iApply (wp_par heapN N (λ _, True%I) (λ _, True%I)); eauto.
+      iFrame "Hh"; iSplitL "H1"; [|iSplitL "H2"; [|iIntros {_ _} "_"; by iNext]];
+        iApply worker_safe; by iSplit.
 Qed.
 End client.
 
@@ -81,11 +63,9 @@ Section ClosedProofs.
 
   Lemma client_safe_closed σ : {{ ownP σ : iProp }} client {{ λ v, True }}.
   Proof.
-    apply ht_alt. rewrite (heap_alloc (nroot .@ "Barrier")); last done.
-    apply wp_strip_pvs, exist_elim=> ?. rewrite and_elim_l.
-    rewrite -(client_safe (nroot .@ "Barrier") (nroot .@ "Heap")) //.
-    (* This, too, should be automated. *)
-    by apply ndot_ne_disjoint.
+    iIntros "! Hσ".
+    iPvs (heap_alloc (nroot .@ "Barrier")) "Hσ" as {h} "[#Hh _]"; first done.
+    iApply (client_safe (nroot .@ "Barrier") (nroot .@ "Heap")); auto with ndisj.
   Qed.
 
   Print Assumptions client_safe_closed.
