heap_lang/lib/spawn.v
@@ -1,6 +1,7 @@
 From iris.program_logic Require Export global_functor.
 From iris.heap_lang Require Export heap.
-From iris.heap_lang Require Import wp_tactics notation.
+From iris.proofmode Require Import invariants ghost_ownership.
+From iris.heap_lang Require Import proofmode notation.
 Import uPred.
 
 Definition spawn : val :=
@@ -33,11 +34,14 @@ Context (heapN N : namespace).
 Local Notation iProp := (iPropG heap_lang Σ).
 
 Definition spawn_inv (γ : gname) (l : loc) (Ψ : val → iProp) : iProp :=
-  (∃ lv, l ↦ lv ★ (lv = InjLV #0 ∨ ∃ v, lv = InjRV v ★ (Ψ v ∨ own γ (Excl ()))))%I.
+  (∃ lv, l ↦ lv ★ (lv = InjLV #0 ∨
+                   ∃ v, lv = InjRV v ★ (Ψ v ∨ own γ (Excl ()))))%I.
 
 Definition join_handle (l : loc) (Ψ : val → iProp) : iProp :=
   (■ (heapN ⊥ N) ★ ∃ γ, heap_ctx heapN ★ own γ (Excl ()) ★
                         inv N (spawn_inv γ l Ψ))%I.
+
+Typeclasses Opaque join_handle.
 
 Global Instance spawn_inv_ne n γ l :
   Proper (pointwise_relation val (dist n) ==> dist n) (spawn_inv γ l).
@@ -53,65 +57,36 @@ Lemma spawn_spec (Ψ : val → iProp) e (f : val) (Φ : val → iProp) :
   (heap_ctx heapN ★ WP f #() {{ Ψ }} ★ ∀ l, join_handle l Ψ -★ Φ (%l))
   ⊢ WP spawn e {{ Φ }}.
 Proof.
-  intros Hval Hdisj. rewrite /spawn. ewp (by eapply wp_value). wp_let.
-  wp eapply wp_alloc; eauto with I.
-  apply forall_intro=>l. apply wand_intro_l. wp_let.
-  rewrite (forall_elim l). eapply sep_elim_True_l.
-  { by eapply (own_alloc (Excl ())). }
-  rewrite !pvs_frame_r. eapply wp_strip_pvs. rewrite !sep_exist_r.
-  apply exist_elim=>γ.
-  (* TODO: Figure out a better way to say "I want to establish ▷ spawn_inv". *)
-  trans (heap_ctx heapN ★ WP f #() {{ Ψ }} ★ (join_handle l Ψ -★ Φ (%l)%V) ★
-         own γ (Excl ()) ★ ▷ (spawn_inv γ l Ψ))%I.
-  { ecancel [ WP _ {{ _ }}; _ -★ _; heap_ctx _; own _ _]%I.
-    rewrite -later_intro /spawn_inv -(exist_intro (InjLV #0)).
-    cancel [l ↦ InjLV #0]%I. by apply or_intro_l', const_intro. }
-  rewrite (inv_alloc N) // !pvs_frame_l. eapply wp_strip_pvs.
-  ewp eapply wp_fork. rewrite [heap_ctx _]always_sep_dup [inv _ _]always_sep_dup.
-  sep_split left: [_ -★ _; inv _ _; own _ _; heap_ctx _]%I.
-  - wp_seq. rewrite -pvs_intro. eapply wand_apply_l; [done..|].
-    rewrite /join_handle. rewrite const_equiv // left_id -(exist_intro γ).
-    solve_sep_entails.
-  - wp_focus (f _). rewrite wp_frame_r wp_frame_l.
-    rewrite (of_to_val e) //. apply wp_mono=>v.
-    eapply (inv_fsa (wp_fsa _)) with (N0:=N);
-      rewrite /= ?to_of_val; eauto with I ndisj.
-    apply wand_intro_l. rewrite /spawn_inv {1}later_exist !sep_exist_r.
-    apply exist_elim=>lv. rewrite later_sep.
-    eapply wp_store; rewrite /= ?to_of_val; eauto with I ndisj.
-    cancel [▷ (l ↦ lv)]%I. strip_later. apply wand_intro_l.
-    rewrite right_id -later_intro -{2}[(∃ _, _ ↦ _ ★ _)%I](exist_intro (InjRV v)).
-    ecancel [l ↦ _]%I. apply or_intro_r'. rewrite sep_elim_r sep_elim_r sep_elim_l.
-    rewrite -(exist_intro v). rewrite const_equiv // left_id. apply or_intro_l.
+  iIntros {<-%of_to_val ?} "(#Hh&Hf&HΦ)". rewrite /spawn.
+  wp_let; wp_alloc l as "Hl"; wp_let.
+  iPvs (own_alloc (Excl ())) as {γ} "Hγ"; first done.
+  iPvs (inv_alloc N _ (spawn_inv γ l Ψ)) "[Hl]" as "#?"; first done.
+  { iNext. iExists (InjLV #0). iFrame "Hl". by iLeft. }
+  wp_apply wp_fork. iSplitR "Hf".
+  - wp_seq. iPvsIntro. iApply "HΦ"; rewrite /join_handle. iSplit; first done.
+    iExists γ. iFrame "Hγ"; by iSplit.
+  - wp_focus (f _). iApply wp_wand_l; iFrame "Hf"; iIntros {v} "Hv".
+    iInv N as "Hinv"; first wp_done; iDestruct "Hinv" as {v'} "[Hl _]".
+    wp_store. iSplit; [iNext|done].
+    iExists (InjRV v); iFrame "Hl"; iRight; iExists v; iSplit; [done|by iLeft].
 Qed.
 
 Lemma join_spec (Ψ : val → iProp) l (Φ : val → iProp) :
-  (join_handle l Ψ ★ ∀ v, Ψ v -★ Φ v)
-  ⊢ WP join (%l) {{ Φ }}.
+  (join_handle l Ψ ★ ∀ v, Ψ v -★ Φ v) ⊢ WP join (%l) {{ Φ }}.
 Proof.
-  wp_rec. wp_focus (! _)%E.
-  rewrite {1}/join_handle sep_exist_l !sep_exist_r. apply exist_elim=>γ.
-  rewrite -!assoc. apply const_elim_sep_l=>Hdisj.
-  eapply (inv_fsa (wp_fsa _)) with (N0:=N); simpl; eauto with I ndisj.
-  apply wand_intro_l. rewrite /spawn_inv {1}later_exist !sep_exist_r.
-  apply exist_elim=>lv.
-  wp eapply wp_load; eauto with I ndisj. cancel [l ↦ lv]%I.
-  apply wand_intro_l. rewrite -later_intro -[X in _ ⊢ (X ★ _)](exist_intro lv).
-  cancel [l ↦ lv]%I. rewrite sep_or_r. apply or_elim.
-  - (* Case 1 : nothing sent yet, we wait. *)
-    rewrite -or_intro_l. apply const_elim_sep_l=>-> {lv}.
-    rewrite (const_equiv (_ = _)) // left_id. wp_case.
-    wp_seq. rewrite -always_wand_impl always_elim.
-    rewrite !assoc. eapply wand_apply_r'; first done.
-    rewrite -(exist_intro γ) const_equiv //. solve_sep_entails.
-  - rewrite [(_ ★ □ _)%I]sep_elim_l -or_intro_r !sep_exist_r. apply exist_mono=>v.
-    rewrite -!assoc. apply const_elim_sep_l=>->{lv}. rewrite const_equiv // left_id.
-    rewrite sep_or_r. apply or_elim; last first.
-    { (* contradiction: we have the token twice. *)
-      rewrite [(heap_ctx _ ★ _)%I]sep_elim_r !assoc. rewrite -own_op own_valid_l.
-      rewrite -!assoc discrete_valid. apply const_elim_sep_l=>-[]. }
-    rewrite -or_intro_r. ecancel [own _ _].
-    wp_case. wp_let. ewp (eapply wp_value; wp_done).
-    rewrite (forall_elim v). rewrite !assoc. eapply wand_apply_r'; eauto with I.
+  rewrite /join_handle; iIntros "[[% H] Hv]"; iDestruct "H" as {γ} "(#?&Hγ&#?)".
+  iLöb "Hγ Hv" as "IH". wp_rec. wp_focus (! _)%E.
+  iInv N as "Hinv"; iDestruct "Hinv" as {v} "[Hl Hinv]".
+  wp_load. iDestruct "Hinv" as "[%|Hinv]"; subst.
+  - iSplitL "Hl"; [iNext; iExists _; iFrame "Hl"; by iLeft|].
+    wp_case. wp_seq. iApply "IH" "Hγ Hv".
+  - iDestruct "Hinv" as {v'} "[% [HΨ|Hγ']]"; subst.
+    + iSplitL "Hl Hγ".
+      { iNext. iExists _; iFrame "Hl"; iRight.
+        iExists _; iSplit; [done|by iRight]. }
+      wp_case. wp_let. iPvsIntro. by iApply "Hv".
+    + iCombine "Hγ" "Hγ'" as "Hγ". by iDestruct own_valid "Hγ" as "%".
 Qed.
 End proof.
+
+Typeclasses Opaque join_handle.
