tests/joining_existentials.v
@@ -1,11 +1,12 @@
-From iris.program_logic Require Import saved_one_shot hoare tactics.
+From iris.program_logic Require Import saved_one_shot hoare.
 From iris.heap_lang.lib.barrier Require Import proof specification.
-From iris.heap_lang Require Import notation par.
+From iris.heap_lang Require Import notation par proofmode.
+From iris.proofmode Require Import invariants.
 Import uPred.
 
 Definition client eM eW1 eW2 : expr [] :=
-  (let: "b" := newbarrier #() in (eM ;; ^signal '"b") ||
-                              ((^wait '"b" ;; eW1) || (^wait '"b" ;; eW2))).
+  let: "b" := newbarrier #() in
+  (eM ;; ^signal '"b") || ((^wait '"b" ;; eW1) || (^wait '"b" ;; eW2)).
 
 Section proof.
 Context (G : cFunctor).
@@ -14,92 +15,67 @@ Context (heapN N : namespace).
 Local Notation iProp := (iPropG heap_lang Σ).
 Local Notation X := (G iProp).
 
-Definition barrier_res γ (P : X → iProp) : iProp :=
-  (∃ x:X, one_shot_own γ x ★ P x)%I.
+Definition barrier_res γ (Φ : X → iProp) : iProp :=
+  (∃ x, one_shot_own γ x ★ Φ x)%I.
 
-
-Lemma worker_spec e γ l (P Q : X → iProp) (R : iProp) :
-  R ⊢ (∀ x, {{ P x }} e {{ λ _, Q x }}) →
-  R ⊢ (recv heapN N l (barrier_res γ P)) →
-  R ⊢ WP wait (%l) ;; e {{ λ _, barrier_res γ Q }}.
+Lemma worker_spec e γ l (Φ Ψ : X → iProp) :
+  (recv heapN N l (barrier_res γ Φ) ★ ∀ x, {{ Φ x }} e {{ λ _, Ψ x }})
+  ⊢ WP wait (%l) ;; e {{ λ _, barrier_res γ Ψ }}.
 Proof.
-  intros He HΦ. rewrite -[R](idemp (∧)%I) {1}He HΦ always_and_sep_l {He HΦ}.
-  ewp (eapply wait_spec). ecancel [recv _ _ l _]. apply wand_intro_r. wp_seq.
-  rewrite /barrier_res sep_exist_l. apply exist_elim=>x.
-  rewrite (forall_elim x) /ht always_elim impl_wand !assoc.
-  to_front [P x; _ -★ _]%I. rewrite wand_elim_r !wp_frame_r.
-  apply wp_mono=>v. by rewrite -(exist_intro x) comm.
+  iIntros "[Hl #He]". wp_apply wait_spec; iFrame "Hl".
+  iIntros "Hγ"; iDestruct "Hγ" as {x} "[#Hγ Hx]".
+  wp_seq. iApply wp_wand_l. iSplitR; [|by iApply "He" "!"].
+  iIntros {v} "?"; iExists x; by iSplit.
 Qed.
 
-Context (P' : iProp) (P P1 P2 Q Q1 Q2 : X -n> iProp).
-Context {P_split : ∀ x:X, P x ⊢ (P1 x ★ P2 x)}.
-Context {Q_join  : ∀ x:X, (Q1 x ★ Q2 x) ⊢ Q x}.
+Context (P : iProp) (Φ Φ1 Φ2 Ψ Ψ1 Ψ2 : X -n> iProp).
+Context {Φ_split : ∀ x, Φ x ⊢ (Φ1 x ★ Φ2 x)}.
+Context {Ψ_join  : ∀ x, (Ψ1 x ★ Ψ2 x) ⊢ Ψ x}.
 
-Lemma P_res_split γ :
-  barrier_res γ P ⊢ (barrier_res γ P1 ★ barrier_res γ P2).
+Lemma P_res_split γ : barrier_res γ Φ ⊢ (barrier_res γ Φ1 ★ barrier_res γ Φ2).
 Proof.
-  rewrite /barrier_res. apply exist_elim=>x. do 2 rewrite -(exist_intro x).
-  rewrite P_split {1}[one_shot_own _ _]always_sep_dup.
-  solve_sep_entails.
+  iIntros "Hγ"; iDestruct "Hγ" as {x} "[#Hγ Hx]".
+  iDestruct Φ_split "Hx" as "[H1 H2]". by iSplitL "H1"; iExists x; iSplit.
 Qed.
 
-Lemma Q_res_join γ :
-  (barrier_res γ Q1 ★ barrier_res γ Q2) ⊢ ▷ barrier_res γ Q.
+Lemma Q_res_join γ : (barrier_res γ Ψ1 ★ barrier_res γ Ψ2) ⊢ ▷ barrier_res γ Ψ.
 Proof.
-  rewrite /barrier_res sep_exist_r. apply exist_elim=>x1.
-  rewrite sep_exist_l. apply exist_elim=>x2.
-  rewrite [one_shot_own γ x1]always_sep_dup.
-  to_front [one_shot_own γ x1; one_shot_own γ x2]. rewrite one_shot_agree.
-  strip_later. rewrite -(exist_intro x1) -Q_join.
-  ecancel [one_shot_own γ _; Q1 _].
-  eapply (eq_rewrite x2 x1 (λ x, Q2 x)); last by eauto with I.
-  { (* FIXME typeclass search should find this. *)
-    apply cofe_mor_ne. }
-  rewrite eq_sym. eauto with I.
+  iIntros "[Hγ Hγ']";
+  iDestruct "Hγ" as {x} "[#Hγ Hx]"; iDestruct "Hγ'" as {x'} "[#Hγ' Hx']".
+  iDestruct (one_shot_agree γ x x') "- !" as "Hxx"; first (by iSplit).
+  iNext. iRewrite -"Hxx" in "Hx'".
+  iExists x; iFrame "Hγ". iApply Ψ_join; by iSplitL "Hx".
 Qed.
 
-Lemma client_spec (eM eW1 eW2 : expr []) (eM' eW1' eW2' : expr ("b" :b: [])) (R : iProp) :
+Lemma client_spec_new (eM eW1 eW2 : expr []) (eM' eW1' eW2' : expr ("b" :b: [])) :
   heapN ⊥ N → eM' = wexpr' eM → eW1' = wexpr' eW1 → eW2' = wexpr' eW2 →
-  R ⊢ ({{ P' }} eM {{ λ _, ∃ x, P x }}) →
-  R ⊢ (∀ x, {{ P1 x }} eW1 {{ λ _, Q1 x }}) →
-  R ⊢ (∀ x, {{ P2 x }} eW2 {{ λ _, Q2 x }}) →
-  R ⊢ heap_ctx heapN →
-  R ⊢ P' →
-  R ⊢ WP client eM' eW1' eW2' {{ λ _, ∃ γ, barrier_res γ Q }}.
+  (heap_ctx heapN ★ P
+  ★ {{ P }} eM {{ λ _, ∃ x, Φ x }}
+  ★ (∀ x, {{ Φ1 x }} eW1 {{ λ _, Ψ1 x }})
+  ★ (∀ x, {{ Φ2 x }} eW2 {{ λ _, Ψ2 x }}))
+  ⊢ WP client eM' eW1' eW2' {{ λ _, ∃ γ, barrier_res γ Ψ }}.
 Proof.
-  intros HN -> -> -> HeM HeW1 HeW2 Hheap HP'.
-  rewrite -4!{1}[R](idemp (∧)%I) {1}HeM {1}HeW1 {1}HeW2 {1}Hheap {1}HP' !always_and_sep_l {Hheap} /client.
-  to_front []. rewrite one_shot_alloc !pvs_frame_r !sep_exist_r.
-  apply wp_strip_pvs, exist_elim=>γ. rewrite {1}[heap_ctx _]always_sep_dup.
-  (ewp (eapply (newbarrier_spec heapN N (barrier_res γ P)))); last done.
-  cancel [heap_ctx heapN]. apply forall_intro=>l. apply wand_intro_r.
-  set (workers_post (v : val) := (barrier_res γ Q1 ★ barrier_res γ Q2)%I).
-  wp_let. (ewp (eapply wp_par with (Ψ1 := λ _, True%I) (Ψ2 := workers_post))); last first.
-  { done. } (* FIXME why does this simple goal even appear? *)
-  rewrite {1}[heap_ctx _]always_sep_dup. cancel [heap_ctx heapN].
-  sep_split left: [one_shot_pending γ; send _ _ _ _ ; P'; {{ _ }} eM {{ _ }}]%I.
-  { (* Main thread. *)
-    wp_focus eM. rewrite /ht always_elim impl_wand wand_elim_r !wp_frame_l.
-    apply wp_mono=>v. wp_seq. rewrite !sep_exist_l. apply exist_elim=>x.
-    rewrite (one_shot_init _ γ x) !pvs_frame_r. apply wp_strip_pvs.
-    ewp (eapply signal_spec). ecancel [send _ _ _ _].
-    by rewrite /barrier_res -(exist_intro x). }
-  sep_split right: [].
-  - (* Worker threads. *)
-    rewrite recv_mono; last exact: P_res_split. rewrite (recv_split _ _ ⊤) //.
-    rewrite ?pvs_frame_r !pvs_frame_l. apply wp_strip_pvs.
-    (ewp (eapply wp_par with (Ψ1 := λ _, barrier_res γ Q1) (Ψ2 := λ _, barrier_res γ Q2))); last first.
-    { done. } ecancel [heap_ctx _].
-    sep_split left: [recv _ _ _ (barrier_res γ P1); ∀ _, {{ _ }} eW1 {{ _ }}]%I.
-    { eapply worker_spec; eauto with I. }
-    sep_split left: [recv _ _ _ (barrier_res γ P2); ∀ _, {{ _ }} eW2 {{ _ }}]%I.
-    { eapply worker_spec; eauto with I. }
-    rewrite /workers_post. do 2 apply forall_intro=>_. 
-    (* FIXME: this should work: rewrite -later_intro. *)
-    apply wand_intro_r. rewrite -later_intro. solve_sep_entails.
-  - (* Merging. *)
-    rewrite /workers_post. do 2 apply forall_intro=>_. apply wand_intro_r.
-    rewrite !left_id Q_res_join. strip_later. by rewrite -(exist_intro γ).
+  iIntros {HN -> -> ->} "/= (#Hh&HP&#He&#He1&#He2)"; rewrite /client.
+  iPvs one_shot_alloc as {γ} "Hγ".
+  wp_apply (newbarrier_spec heapN N (barrier_res γ Φ)); auto.
+  iFrame "Hh". iIntros {l} "[Hr Hs]".
+  set (workers_post (v : val) := (barrier_res γ Ψ1 ★ barrier_res γ Ψ2)%I).
+  wp_let. wp_apply (wp_par _ _ (λ _, True)%I workers_post); first done.
+  iFrame "Hh". iSplitL "HP Hs Hγ"; [|iSplitL "Hr"].
+  - wp_focus eM. iApply wp_wand_l; iSplitR "HP"; [|iApply "He" "HP"].
+    iIntros {v} "HP"; iDestruct "HP" as {x} "HP". wp_let.
+    iPvs (one_shot_init _ _ x) "Hγ" as "Hx".
+    iApply signal_spec; iFrame "Hs"; iSplit; last done.
+    iExists x; by iSplitL "Hx".
+  - iDestruct recv_weaken "[] Hr" as "Hr".
+    { iIntros "?". by iApply P_res_split "-". }
+    iPvs recv_split "Hr" as "[H1 H2]"; first done.
+    wp_apply (wp_par _ _ (λ _, barrier_res γ Ψ1)%I
+      (λ _, barrier_res γ Ψ2)%I); first done.
+    iSplit; [done|]; iSplitL "H1"; [|iSplitL "H2"].
+    + by iApply worker_spec; iSplitL "H1".
+    + by iApply worker_spec; iSplitL "H2".
+    + iIntros {v1 v2} "?". by iNext.
+  - iIntros {_ v} "[_ H]"; iPoseProof Q_res_join "H". by iNext; iExists γ.
 Qed.
-
 End proof.
