heap_lang/proofmode.v
@@ -1,0 +1,176 @@
+From iris.proofmode Require Import coq_tactics.
+From iris.proofmode Require Export weakestpre.
+From iris.heap_lang Require Export wp_tactics heap.
+Import uPred.
+
+Ltac strip_later ::= iNext.
+
+Section heap.
+Context {Σ : gFunctors} `{heapG Σ}.
+Implicit Types N : namespace.
+Implicit Types P Q : iPropG heap_lang Σ.
+Implicit Types Φ : val → iPropG heap_lang Σ.
+Implicit Types Δ : envs (iResR heap_lang (globalF Σ)).
+
+Global Instance sep_destruct_mapsto l q v :
+  SepDestruct false (l ↦{q} v) (l ↦{q/2} v) (l ↦{q/2} v).
+Proof. by rewrite /SepDestruct heap_mapsto_op_split. Qed.
+
+Lemma tac_wp_alloc Δ Δ' N E j e v Φ :
+  to_val e = Some v → 
+  Δ ⊢ heap_ctx N → nclose N ⊆ E →
+  StripLaterEnvs Δ Δ' →
+  (∀ l, ∃ Δ'',
+    envs_app false (Esnoc Enil j (l ↦ v)) Δ' = Some Δ'' ∧ Δ'' ⊢ Φ (LocV l)) →
+  Δ ⊢ WP Alloc e @ E {{ Φ }}.
+Proof.
+  intros ???? HΔ; eapply wp_alloc; eauto.
+  rewrite strip_later_env_sound; apply later_mono, forall_intro=> l.
+  destruct (HΔ l) as (Δ''&?&HΔ'). rewrite envs_app_sound //; simpl.
+  by rewrite right_id HΔ'.
+Qed.
+
+Lemma tac_wp_load Δ Δ' N E i l q v Φ :
+  Δ ⊢ heap_ctx N → nclose N ⊆ E →
+  StripLaterEnvs Δ Δ' →
+  envs_lookup i Δ' = Some (false, l ↦{q} v)%I →
+  Δ' ⊢ Φ v →
+  Δ ⊢ WP Load (Loc l) @ E {{ Φ }}.
+Proof.
+  intros. eapply wp_load; eauto.
+  rewrite strip_later_env_sound -later_sep envs_lookup_split //; simpl.
+  by apply later_mono, sep_mono_r, wand_mono.
+Qed.
+
+Lemma tac_wp_store Δ Δ' Δ'' N E i l v e v' Φ :
+  to_val e = Some v' →
+  Δ ⊢ heap_ctx N → nclose N ⊆ E →
+  StripLaterEnvs Δ Δ' →
+  envs_lookup i Δ' = Some (false, l ↦ v)%I →
+  envs_simple_replace i false (Esnoc Enil i (l ↦ v')) Δ' = Some Δ'' →
+  Δ'' ⊢ Φ (LitV LitUnit) → Δ ⊢ WP Store (Loc l) e @ E {{ Φ }}.
+Proof.
+  intros. eapply wp_store; eauto.
+  rewrite strip_later_env_sound -later_sep envs_simple_replace_sound //; simpl.
+  rewrite right_id. by apply later_mono, sep_mono_r, wand_mono.
+Qed.
+
+Lemma tac_wp_cas_fail Δ Δ' N E i l q v e1 v1 e2 v2 Φ :
+  to_val e1 = Some v1 → to_val e2 = Some v2 →
+  Δ ⊢ heap_ctx N → nclose N ⊆ E →
+  StripLaterEnvs Δ Δ' →
+  envs_lookup i Δ' = Some (false, l ↦{q} v)%I → v ≠ v1 →
+  Δ' ⊢ Φ (LitV (LitBool false)) →
+  Δ ⊢ WP CAS (Loc l) e1 e2 @ E {{ Φ }}.
+Proof.
+  intros. eapply wp_cas_fail; eauto.
+  rewrite strip_later_env_sound -later_sep envs_lookup_split //; simpl.
+  by apply later_mono, sep_mono_r, wand_mono.
+Qed.
+
+Lemma tac_wp_cas_suc Δ Δ' Δ'' N E i l e1 v1 e2 v2 Φ :
+  to_val e1 = Some v1 → to_val e2 = Some v2 →
+  Δ ⊢ heap_ctx N → nclose N ⊆ E →
+  StripLaterEnvs Δ Δ' →
+  envs_lookup i Δ' = Some (false, l ↦ v1)%I →
+  envs_simple_replace i false (Esnoc Enil i (l ↦ v2)) Δ' = Some Δ'' →
+  Δ'' ⊢ Φ (LitV (LitBool true)) → Δ ⊢ WP CAS (Loc l) e1 e2 @ E {{ Φ }}.
+Proof.
+  intros. eapply wp_cas_suc; eauto.
+  rewrite strip_later_env_sound -later_sep envs_simple_replace_sound //; simpl.
+  rewrite right_id. by apply later_mono, sep_mono_r, wand_mono.
+Qed.
+End heap.
+
+Tactic Notation "wp_apply" open_constr(lem) :=
+  match goal with
+  | |- _ ⊢ wp ?E ?e ?Q => reshape_expr e ltac:(fun K e' =>
+    wp_bind K; iApply lem; try iNext)
+  end.
+
+Tactic Notation "wp_apply" open_constr(lem) constr(Hs) :=
+  match goal with
+  | |- _ ⊢ wp ?E ?e ?Q => reshape_expr e ltac:(fun K e' =>
+    wp_bind K; iApply lem Hs; try iNext)
+  end.
+
+Tactic Notation "wp_alloc" ident(l) "as" constr(H) :=
+  match goal with
+  | |- _ ⊢ wp ?E ?e ?Q => reshape_expr e ltac:(fun K e' =>
+    match eval hnf in e' with
+    | Alloc ?e =>
+       wp_bind K; eapply tac_wp_alloc with _ _ H _;
+         [wp_done || fail 2 "wp_alloc:" e "not a value"
+         |iAssumption || fail 2 "wp_alloc: cannot find heap_ctx"
+         |done || eauto with ndisj
+         |apply _
+         |intros l; eexists; split;
+           [env_cbv; reflexivity || fail 2 "wp_alloc:" H "not fresh"
+           |wp_finish]]
+    end)
+  end.
+Tactic Notation "wp_alloc" ident(l) := let H := iFresh in wp_alloc l as H.
+
+Tactic Notation "wp_load" :=
+  match goal with
+  | |- _ ⊢ wp ?E ?e ?Q => reshape_expr e ltac:(fun K e' =>
+    match eval hnf in e' with
+    | Load (Loc ?l) =>
+       wp_bind K; eapply tac_wp_load;
+         [iAssumption || fail 2 "wp_load: cannot find heap_ctx"
+         |done || eauto with ndisj
+         |apply _
+         |iAssumptionCore || fail 2 "wp_cas_fail: cannot find" l "↦ ?"
+         |wp_finish]
+    end)
+  end.
+
+Tactic Notation "wp_store" :=
+  match goal with
+  | |- _ ⊢ wp ?E ?e ?Q => reshape_expr e ltac:(fun K e' =>
+    match eval hnf in e' with
+    | Store ?l ?e =>
+       wp_bind K; eapply tac_wp_store;
+         [wp_done || fail 2 "wp_store:" e "not a value"
+         |iAssumption || fail 2 "wp_store: cannot find heap_ctx"
+         |done || eauto with ndisj
+         |apply _
+         |iAssumptionCore || fail 2 "wp_store: cannot find" l "↦ ?"
+         |env_cbv; reflexivity
+         |wp_finish]
+    end)
+  end.
+
+Tactic Notation "wp_cas_fail" :=
+  match goal with
+  | |- _ ⊢ wp ?E ?e ?Q => reshape_expr e ltac:(fun K e' =>
+    match eval hnf in e' with
+    | CAS (Loc ?l) ?e1 ?e2 =>
+       wp_bind K; eapply tac_wp_cas_fail;
+         [wp_done || fail 2 "wp_cas_fail:" e1 "not a value"
+         |wp_done || fail 2 "wp_cas_fail:" e2 "not a value"
+         |iAssumption || fail 2 "wp_cas_fail: cannot find heap_ctx"
+         |done || eauto with ndisj
+         |apply _
+         |iAssumptionCore || fail 2 "wp_cas_fail: cannot find" l "↦ ?"
+         |try discriminate
+         |wp_finish]
+    end)
+  end.
+
+Tactic Notation "wp_cas_suc" :=
+  match goal with
+  | |- _ ⊢ wp ?E ?e ?Q => reshape_expr e ltac:(fun K e' =>
+    match eval hnf in e' with
+    | CAS (Loc ?l) ?e1 ?e2 =>
+       wp_bind K; eapply tac_wp_cas_suc;
+         [wp_done || fail 2 "wp_cas_suc:" e1 "not a value"
+         |wp_done || fail 2 "wp_cas_suc:" e1 "not a value"
+         |iAssumption || fail 2 "wp_cas_suc: cannot find heap_ctx"
+         |done || eauto with ndisj
+         |apply _
+         |iAssumptionCore || fail 2 "wp_cas_suc: cannot find" l "↦ ?"
+         |env_cbv; reflexivity
+         |wp_finish]
+    end)
+  end.
