program_logic/viewshifts.v
@@ -1,5 +1,6 @@
 From iris.program_logic Require Import ownership.
 From iris.program_logic Require Export pviewshifts invariants ghost_ownership.
+From iris.proofmode Require Import pviewshifts.
 Import uPred.
 
 Definition vs {Λ Σ} (E1 E2 : coPset) (P Q : iProp Λ Σ) : iProp Λ Σ :=
@@ -23,10 +24,7 @@ Implicit Types P Q R : iProp Λ Σ.
 Implicit Types N : namespace.
 
 Lemma vs_alt E1 E2 P Q : P ⊢ (|={E1,E2}=> Q) → P ={E1,E2}=> Q.
-Proof.
-  intros; rewrite -{1}always_const. apply: always_intro. apply impl_intro_l.
-  by rewrite always_const right_id.
-Qed.
+Proof. iIntros {Hvs} "! ?". by iApply Hvs. Qed.
 
 Global Instance vs_ne E1 E2 n :
   Proper (dist n ==> dist n ==> dist n) (@vs Λ Σ E1 E2).
@@ -44,44 +42,35 @@ Global Instance vs_mono' E1 E2 :
 Proof. solve_proper. Qed.
 
 Lemma vs_false_elim E1 E2 P : False ={E1,E2}=> P.
-Proof. apply vs_alt, False_elim. Qed.
+Proof. iIntros "! []". Qed.
 Lemma vs_timeless E P : TimelessP P → ▷ P ={E}=> P.
-Proof. by intros ?; apply vs_alt, pvs_timeless. Qed.
+Proof. iIntros {?} "! HP". by iApply pvs_timeless. Qed.
 
 Lemma vs_transitive E1 E2 E3 P Q R :
   E2 ⊆ E1 ∪ E3 → ((P ={E1,E2}=> Q) ∧ (Q ={E2,E3}=> R)) ⊢ (P ={E1,E3}=> R).
 Proof.
-  intros; rewrite -always_and; apply: always_intro. apply impl_intro_l.
-  rewrite always_and assoc (always_elim (P → _)) impl_elim_r.
-  by rewrite pvs_impl_r; apply pvs_trans.
+  iIntros {?} "#[HvsP HvsQ] ! HP".
+  iPvs "HvsP" "! HP" as "HQ"; first done. by iApply "HvsQ" "!".
 Qed.
 
 Lemma vs_transitive' E P Q R : ((P ={E}=> Q) ∧ (Q ={E}=> R)) ⊢ (P ={E}=> R).
 Proof. apply vs_transitive; set_solver. Qed.
 Lemma vs_reflexive E P : P ={E}=> P.
-Proof. apply vs_alt, pvs_intro. Qed.
+Proof. iIntros "! HP"; by iPvsIntro. Qed.
 
 Lemma vs_impl E P Q : □ (P → Q) ⊢ (P ={E}=> Q).
-Proof.
-  apply always_intro', impl_intro_l.
-  by rewrite always_elim impl_elim_r -pvs_intro.
-Qed.
+Proof. iIntros "#HPQ ! HP". iPvsIntro. by iApply "HPQ". Qed.
 
 Lemma vs_frame_l E1 E2 P Q R : (P ={E1,E2}=> Q) ⊢ (R ★ P ={E1,E2}=> R ★ Q).
-Proof.
-  apply always_intro', impl_intro_l.
-  rewrite -pvs_frame_l always_and_sep_r -always_wand_impl -assoc.
-  by rewrite always_elim wand_elim_r.
-Qed.
+Proof. iIntros "#Hvs ! [HR HP]". iFrame "HR". by iApply "Hvs". Qed.
 
 Lemma vs_frame_r E1 E2 P Q R : (P ={E1,E2}=> Q) ⊢ (P ★ R ={E1,E2}=> Q ★ R).
-Proof. rewrite !(comm _ _ R); apply vs_frame_l. Qed.
+Proof. iIntros "#Hvs ! [HP HR]". iFrame "HR". by iApply "Hvs". Qed.
 
 Lemma vs_mask_frame E1 E2 Ef P Q :
   Ef ⊥ E1 ∪ E2 → (P ={E1,E2}=> Q) ⊢ (P ={E1 ∪ Ef,E2 ∪ Ef}=> Q).
 Proof.
-  intros ?; apply always_intro', impl_intro_l; rewrite (pvs_mask_frame _ _ Ef)//.
-  by rewrite always_elim impl_elim_r.
+  iIntros {?} "#Hvs ! HP". iApply pvs_mask_frame; auto. by iApply "Hvs".
 Qed.
 
 Lemma vs_mask_frame' E Ef P Q : Ef ⊥ E → (P ={E}=> Q) ⊢ (P ={E ∪ Ef}=> Q).
@@ -90,18 +79,12 @@ Proof. intros; apply vs_mask_frame; set_solver. Qed.
 Lemma vs_inv N E P Q R :
   nclose N ⊆ E → (inv N R ★ (▷ R ★ P ={E ∖ nclose N}=> ▷ R ★ Q)) ⊢ (P ={E}=> Q).
 Proof.
-  intros; apply: always_intro. apply impl_intro_l.
-  rewrite always_and_sep_r assoc [(P ★ _)%I]comm -assoc.
-  eapply pvs_inv; [by eauto with I..|].
-  rewrite sep_elim_r. apply wand_intro_l.
-  (* Oh wow, this is annyoing... *)
-  rewrite assoc -always_and_sep_r'.
-  by rewrite /vs always_elim impl_elim_r.
+  iIntros {?} "#[? Hvs] ! HP". eapply pvs_inv; eauto.
+  iIntros "HR". iApply "Hvs" "!". by iSplitL "HR".
 Qed.
 
 Lemma vs_alloc N P : ▷ P ={N}=> inv N P.
-Proof. by intros; apply vs_alt, inv_alloc. Qed.
-
+Proof. iIntros "! HP". by iApply inv_alloc. Qed.
 End vs.
 
 Section vs_ghost.
@@ -116,8 +99,6 @@ Proof. by intros; apply vs_alt, own_updateP. Qed.
 Lemma vs_update E γ a a' : a ~~> a' → own γ a ={E}=> own γ a'.
 Proof. by intros; apply vs_alt, own_update. Qed.
 
-Lemma vs_own_empty `{Empty A, !CMRAUnit A} E γ :
-  True ={E}=> own γ ∅.
+Lemma vs_own_empty `{Empty A, !CMRAUnit A} E γ : True ={E}=> own γ ∅.
 Proof. by intros; eapply vs_alt, own_empty. Qed.
-
 End vs_ghost.
