proofmode/coq_tactics.v
@@ -1,0 +1,808 @@
+From iris.algebra Require Export upred.
+From iris.algebra Require Import upred_big_op upred_tactics.
+From iris.proofmode Require Export environments.
+From iris.prelude Require Import stringmap.
+Import uPred.
+
+Local Notation "Γ !! j" := (env_lookup j Γ).
+Local Notation "x ← y ; z" := (match y with Some x => z | None => None end).
+Local Notation "' ( x1 , x2 ) ← y ; z" :=
+  (match y with Some (x1,x2) => z | None => None end).
+Local Notation "' ( x1 , x2 , x3 ) ← y ; z" :=
+  (match y with Some (x1,x2,x3) => z | None => None end).
+
+Record envs (M : cmraT) :=
+  Envs { env_persistent : env (uPred M); env_spatial : env (uPred M) }.
+Add Printing Constructor envs.
+Arguments Envs {_} _ _.
+Arguments env_persistent {_} _.
+Arguments env_spatial {_} _.
+
+Record envs_wf {M} (Δ : envs M) := {
+  env_persistent_valid : env_wf (env_persistent Δ);
+  env_spatial_valid : env_wf (env_spatial Δ);
+  envs_disjoint i : env_persistent Δ !! i = None ∨ env_spatial Δ !! i = None
+}.
+
+Coercion of_envs {M} (Δ : envs M) : uPred M :=
+  (■ envs_wf Δ ★ □ Π∧ env_persistent Δ ★ Π★ env_spatial Δ)%I.
+
+Instance envs_dom {M} : Dom (envs M) stringset := λ Δ,
+  dom stringset (env_persistent Δ) ∪ dom stringset (env_spatial Δ).
+
+Definition envs_lookup {M} (i : string) (Δ : envs M) : option (bool * uPred M) :=
+  let (Γp,Γs) := Δ in
+  match env_lookup i Γp with
+  | Some P => Some (true, P) | None => P ← env_lookup i Γs; Some (false, P)
+  end.
+
+Definition envs_delete {M} (i : string) (p : bool) (Δ : envs M) : envs M :=
+  let (Γp,Γs) := Δ in
+  match p with
+  | true => Envs (env_delete i Γp) Γs | false => Envs Γp (env_delete i Γs)
+  end.
+
+Definition envs_lookup_delete {M} (i : string)
+    (Δ : envs M) : option (bool * uPred M * envs M) :=
+  let (Γp,Γs) := Δ in
+  match env_lookup_delete i Γp with
+  | Some (P,Γp') => Some (true, P, Envs Γp' Γs)
+  | None => '(P,Γs') ← env_lookup_delete i Γs; Some (false, P, Envs Γp Γs')
+  end.
+
+Definition envs_app {M} (p : bool)
+    (Γ : env (uPred M)) (Δ : envs M) : option (envs M) :=
+  let (Γp,Γs) := Δ in
+  match p with
+  | true => _ ← env_app Γ Γs; Γp' ← env_app Γ Γp; Some (Envs Γp' Γs)
+  | false => _ ← env_app Γ Γp; Γs' ← env_app Γ Γs; Some (Envs Γp Γs')
+  end.
+
+Definition envs_simple_replace {M} (i : string) (p : bool) (Γ : env (uPred M))
+    (Δ : envs M) : option (envs M) :=
+  let (Γp,Γs) := Δ in
+  match p with
+  | true => _ ← env_app Γ Γs; Γp' ← env_replace i Γ Γp; Some (Envs Γp' Γs)
+  | false => _ ← env_app Γ Γp; Γs' ← env_replace i Γ Γs; Some (Envs Γp Γs')
+  end.
+
+Definition envs_replace {M} (i : string) (p q : bool) (Γ : env (uPred M))
+    (Δ : envs M) : option (envs M) :=
+  if eqb p q then envs_simple_replace i p Γ Δ
+  else envs_app q Γ (envs_delete i p Δ).
+
+(* if [lr = false] then [result = (hyps named js,remainding hyps)],
+   if [lr = true] then [result = (remainding hyps,hyps named js)] *)
+Definition envs_split {M}
+    (lr : bool) (js : list string) (Δ : envs M) : option (envs M * envs M) :=
+  let (Γp,Γs) := Δ in
+  '(Γs1,Γs2) ← env_split js Γs;
+  match lr with
+  | false  => Some (Envs Γp Γs1, Envs Γp Γs2)
+  | true => Some (Envs Γp Γs2, Envs Γp Γs1)
+  end.
+
+Definition envs_persistent {M} (Δ : envs M) :=
+  if env_spatial Δ is Enil then true else false.
+
+(* Coq versions of the tactics *)
+Section tactics.
+Context {M : cmraT}.
+Implicit Types Γ : env (uPred M).
+Implicit Types Δ : envs M.
+Implicit Types P Q : uPred M.
+
+Lemma envs_lookup_delete_Some Δ Δ' i p P :
+  envs_lookup_delete i Δ = Some (p,P,Δ')
+  ↔ envs_lookup i Δ = Some (p,P) ∧ Δ' = envs_delete i p Δ.
+Proof.
+  rewrite /envs_lookup /envs_delete /envs_lookup_delete.
+  destruct Δ as [Γp Γs]; rewrite /= !env_lookup_delete_correct.
+  destruct (Γp !! i), (Γs !! i); naive_solver.
+Qed.
+
+Lemma envs_lookup_sound Δ i p P :
+  envs_lookup i Δ = Some (p,P) →
+  Δ ⊢ ((if p then □ P else P) ★ envs_delete i p Δ).
+Proof.
+  rewrite /envs_lookup /envs_delete /of_envs=>?; apply const_elim_sep_l=> Hwf.
+  destruct Δ as [Γp Γs], (Γp !! i) eqn:?; simplify_eq/=.
+  - rewrite (env_lookup_perm Γp) //= always_and_sep always_sep.
+    ecancel [□ Π∧ _; □ P; Π★ _]%I; apply const_intro.
+    destruct Hwf; constructor;
+      naive_solver eauto using env_delete_wf, env_delete_fresh.
+  - destruct (Γs !! i) eqn:?; simplify_eq/=.
+    rewrite (env_lookup_perm Γs) //=.
+    ecancel [□ Π∧ _; P; Π★ _]%I; apply const_intro.
+    destruct Hwf; constructor;
+      naive_solver eauto using env_delete_wf, env_delete_fresh.
+Qed.
+Lemma envs_lookup_sound' Δ i p P :
+  envs_lookup i Δ = Some (p,P) → Δ ⊢ (P ★ envs_delete i p Δ).
+Proof.
+  intros. rewrite envs_lookup_sound //. by destruct p; rewrite ?always_elim.
+Qed.
+Lemma envs_lookup_persistent_sound Δ i P :
+  envs_lookup i Δ = Some (true,P) → Δ ⊢ (□ P ★ Δ).
+Proof.
+  intros. apply: always_entails_l. by rewrite envs_lookup_sound // sep_elim_l.
+Qed.
+
+Lemma envs_lookup_split Δ i p P :
+  envs_lookup i Δ = Some (p,P) →
+  Δ ⊢ ((if p then □ P else P) ★ ((if p then □ P else P) -★ Δ)).
+Proof.
+  rewrite /envs_lookup /of_envs=>?; apply const_elim_sep_l=> Hwf.
+  destruct Δ as [Γp Γs], (Γp !! i) eqn:?; simplify_eq/=.
+  - rewrite (env_lookup_perm Γp) //= always_and_sep always_sep.
+    rewrite const_equiv // left_id.
+    cancel [□ P]%I. apply wand_intro_l. solve_sep_entails.
+  - destruct (Γs !! i) eqn:?; simplify_eq/=.
+    rewrite (env_lookup_perm Γs) //=. rewrite const_equiv // left_id.
+    cancel [P]. apply wand_intro_l. solve_sep_entails.
+Qed.
+
+Lemma envs_lookup_delete_sound Δ Δ' i p P :
+  envs_lookup_delete i Δ = Some (p,P,Δ') → Δ ⊢ ((if p then □ P else P) ★ Δ')%I.
+Proof. intros [? ->]%envs_lookup_delete_Some. by apply envs_lookup_sound. Qed.
+Lemma envs_lookup_delete_sound' Δ Δ' i p P :
+  envs_lookup_delete i Δ = Some (p,P,Δ') → Δ ⊢ (P ★ Δ')%I.
+Proof. intros [? ->]%envs_lookup_delete_Some. by apply envs_lookup_sound'. Qed.
+
+Lemma envs_app_sound Δ Δ' p Γ :
+  envs_app p Γ Δ = Some Δ' → Δ ⊢ ((if p then □ Π∧ Γ else Π★ Γ) -★ Δ').
+Proof.
+  rewrite /of_envs /envs_app=> ?; apply const_elim_sep_l=> Hwf.
+  destruct Δ as [Γp Γs], p; simplify_eq/=.
+  - destruct (env_app Γ Γs) eqn:Happ,
+      (env_app Γ Γp) as [Γp'|] eqn:?; simplify_eq/=.
+    apply wand_intro_l, sep_intro_True_l; [apply const_intro|].
+    + destruct Hwf; constructor; simpl; eauto using env_app_wf.
+      intros j. apply (env_app_disjoint _ _ _ j) in Happ.
+      naive_solver eauto using env_app_fresh.
+    + rewrite (env_app_perm _ _ Γp') //.
+      rewrite big_and_app always_and_sep always_sep; solve_sep_entails.
+  - destruct (env_app Γ Γp) eqn:Happ,
+      (env_app Γ Γs) as [Γs'|] eqn:?; simplify_eq/=.
+    apply wand_intro_l, sep_intro_True_l; [apply const_intro|].
+    + destruct Hwf; constructor; simpl; eauto using env_app_wf.
+      intros j. apply (env_app_disjoint _ _ _ j) in Happ.
+      naive_solver eauto using env_app_fresh.
+    + rewrite (env_app_perm _ _ Γs') // big_sep_app. solve_sep_entails.
+Qed.
+
+Lemma envs_simple_replace_sound' Δ Δ' i p Γ :
+  envs_simple_replace i p Γ Δ = Some Δ' →
+  envs_delete i p Δ ⊢ ((if p then □ Π∧ Γ else Π★ Γ) -★ Δ')%I.
+Proof.
+  rewrite /envs_simple_replace /envs_delete /of_envs=> ?.
+  apply const_elim_sep_l=> Hwf. destruct Δ as [Γp Γs], p; simplify_eq/=.
+  - destruct (env_app Γ Γs) eqn:Happ,
+      (env_replace i Γ Γp) as [Γp'|] eqn:?; simplify_eq/=.
+    apply wand_intro_l, sep_intro_True_l; [apply const_intro|].
+    + destruct Hwf; constructor; simpl; eauto using env_replace_wf.
+      intros j. apply (env_app_disjoint _ _ _ j) in Happ.
+      destruct (decide (i = j)); try naive_solver eauto using env_replace_fresh.
+    + rewrite (env_replace_perm _ _ Γp') //.
+      rewrite big_and_app always_and_sep always_sep; solve_sep_entails.
+  - destruct (env_app Γ Γp) eqn:Happ,
+      (env_replace i Γ Γs) as [Γs'|] eqn:?; simplify_eq/=.
+    apply wand_intro_l, sep_intro_True_l; [apply const_intro|].
+    + destruct Hwf; constructor; simpl; eauto using env_replace_wf.
+      intros j. apply (env_app_disjoint _ _ _ j) in Happ.
+      destruct (decide (i = j)); try naive_solver eauto using env_replace_fresh.
+    + rewrite (env_replace_perm _ _ Γs') // big_sep_app. solve_sep_entails.
+Qed.
+
+Lemma envs_simple_replace_sound Δ Δ' i p P Γ :
+  envs_lookup i Δ = Some (p,P) → envs_simple_replace i p Γ Δ = Some Δ' →
+  Δ ⊢ ((if p then □ P else P) ★
+       ((if p then □ Π∧ Γ else Π★ Γ) -★ Δ'))%I.
+Proof. intros. by rewrite envs_lookup_sound// envs_simple_replace_sound'//. Qed.
+
+Lemma envs_replace_sound' Δ Δ' i p q Γ :
+  envs_replace i p q Γ Δ = Some Δ' →
+  envs_delete i p Δ ⊢ ((if q then □ Π∧ Γ else Π★ Γ) -★ Δ')%I.
+Proof.
+  rewrite /envs_replace; destruct (eqb _ _) eqn:Hpq.
+  - apply eqb_prop in Hpq as ->. apply envs_simple_replace_sound'.
+  - apply envs_app_sound.
+Qed.
+
+Lemma envs_replace_sound Δ Δ' i p q P Γ :
+  envs_lookup i Δ = Some (p,P) → envs_replace i p q Γ Δ = Some Δ' →
+  Δ ⊢ ((if p then □ P else P) ★
+       ((if q then □ Π∧ Γ else Π★ Γ) -★ Δ'))%I.
+Proof. intros. by rewrite envs_lookup_sound// envs_replace_sound'//. Qed.
+
+Lemma envs_split_sound Δ lr js Δ1 Δ2 :
+  envs_split lr js Δ = Some (Δ1,Δ2) → Δ ⊢ (Δ1 ★ Δ2).
+Proof.
+  rewrite /envs_split /of_envs=> ?; apply const_elim_sep_l=> Hwf.
+  destruct Δ as [Γp Γs], (env_split js _) as [[Γs1 Γs2]|] eqn:?; simplify_eq/=.
+  rewrite (env_split_perm Γs) // big_sep_app {1}always_sep_dup'.
+  destruct lr; simplify_eq/=; cancel [□ Π∧ Γp; □ Π∧ Γp; Π★ Γs1; Π★ Γs2]%I;
+    destruct Hwf; apply sep_intro_True_l; apply const_intro; constructor;
+      naive_solver eauto using env_split_wf_1, env_split_wf_2,
+      env_split_fresh_1, env_split_fresh_2.
+Qed.
+
+Lemma env_special_nil_persistent Δ : envs_persistent Δ = true → PersistentP Δ.
+Proof. intros; destruct Δ as [? []]; simplify_eq/=; apply _. Qed.
+Hint Immediate env_special_nil_persistent : typeclass_instances.
+
+(** * Adequacy *)
+Lemma tac_adequate P : Envs Enil Enil ⊢ P → True ⊢ P.
+Proof.
+  intros <-. rewrite /of_envs /= always_const !right_id.
+  apply const_intro; repeat constructor.
+Qed.
+
+(** * Basic rules *)
+Lemma tac_exact Δ i p P : envs_lookup i Δ = Some (p,P) → Δ ⊢ P.
+Proof. intros. by rewrite envs_lookup_sound' // sep_elim_l. Qed.
+
+Lemma tac_rename Δ Δ' i j p P Q :
+  envs_lookup i Δ = Some (p,P) →
+  envs_simple_replace i p (Esnoc Enil j P) Δ = Some Δ' →
+  Δ' ⊢ Q → Δ ⊢ Q.
+Proof.
+  intros. rewrite envs_simple_replace_sound //.
+  destruct p; simpl; by rewrite right_id wand_elim_r.
+Qed.
+Lemma tac_clear Δ Δ' i p P Q :
+  envs_lookup_delete i Δ = Some (p,P,Δ') → Δ' ⊢ Q → Δ ⊢ Q.
+Proof. intros. by rewrite envs_lookup_delete_sound // sep_elim_r. Qed.
+Lemma tac_clear_spatial Δ Δ1 Δ2 Q :
+  envs_split true [] Δ = Some (Δ1,Δ2) → Δ1 ⊢ Q → Δ ⊢ Q.
+Proof. intros. by rewrite envs_split_sound // sep_elim_l. Qed.
+
+Lemma tac_duplicate Δ Δ' i p j P Q :
+  envs_lookup i Δ = Some (p, P) →
+  p = true →
+  envs_simple_replace i true (Esnoc (Esnoc Enil i P) j P) Δ = Some Δ' →
+  Δ' ⊢ Q → Δ ⊢ Q.
+Proof.
+  intros ? -> ??. rewrite envs_simple_replace_sound //; simpl.
+  by rewrite right_id idemp wand_elim_r.
+Qed.
+
+(** * False *)
+Lemma tac_ex_falso Δ Q : Δ ⊢ False → Δ ⊢ Q.
+Proof. by rewrite -(False_elim Q). Qed.
+
+(** * Pure *)
+Lemma tac_pure_intro Δ (φ : Prop) : φ → Δ ⊢ ■ φ.
+Proof. apply const_intro. Qed.
+
+Class ToPure (P : uPred M) (φ : Prop) := to_pure : P ⊢ ■ φ.
+Arguments to_pure : clear implicits.
+Global Instance to_pure_const φ : ToPure (■ φ) φ.
+Proof. done. Qed.
+Global Instance to_pure_eq {A : cofeT} (a b : A) :
+  Timeless a → ToPure (a ≡ b) (a ≡ b).
+Proof. intros; red. by rewrite timeless_eq. Qed.
+Global Instance to_pure_valid `{CMRADiscrete A} (a : A) : ToPure (✓ a) (✓ a).
+Proof. intros; red. by rewrite discrete_valid. Qed.
+
+Lemma tac_pure Δ Δ' i p P φ Q :
+  envs_lookup_delete i Δ = Some (p, P, Δ') → ToPure P φ →
+  (φ → Δ' ⊢ Q) → Δ ⊢ Q.
+Proof.
+  intros ?? HQ. rewrite envs_lookup_delete_sound' //; simpl.
+  rewrite (to_pure P); by apply const_elim_sep_l.
+Qed.
+
+Lemma tac_pure_revert Δ φ Q : Δ ⊢ (■ φ → Q) → (φ → Δ ⊢ Q).
+Proof. intros HΔ ?. by rewrite HΔ const_equiv // left_id. Qed.
+
+(** * Later *)
+Class StripLaterEnv (Γ1 Γ2 : env (uPred M)) :=
+  strip_later_env : env_Forall2 StripLaterR Γ1 Γ2.
+Global Instance strip_later_env_nil : StripLaterEnv Enil Enil.
+Proof. constructor. Qed.
+Global Instance strip_later_env_snoc Γ1 Γ2 i P Q :
+  StripLaterEnv Γ1 Γ2 → StripLaterR P Q →
+  StripLaterEnv (Esnoc Γ1 i P) (Esnoc Γ2 i Q).
+Proof. by constructor. Qed.
+
+Class StripLaterEnvs (Δ1 Δ2 : envs M) := {
+  strip_later_persistent: StripLaterEnv (env_persistent Δ1) (env_persistent Δ2);
+  strip_later_spatial: StripLaterEnv (env_spatial Δ1) (env_spatial Δ2)
+}.
+Global Instance strip_later_envs Γp1 Γp2 Γs1 Γs2 :
+  StripLaterEnv Γp1 Γp2 → StripLaterEnv Γs1 Γs2 →
+  StripLaterEnvs (Envs Γp1 Γs1) (Envs Γp2 Γs2).
+Proof. by split. Qed.
+Lemma strip_later_env_sound Δ1 Δ2 : StripLaterEnvs Δ1 Δ2 → Δ1 ⊢ ▷ Δ2.
+Proof.
+  intros [Hp Hs]; rewrite /of_envs /= !later_sep -always_later.
+  repeat apply sep_mono; try apply always_mono.
+  - rewrite -later_intro; apply const_mono; destruct 1; constructor;
+      naive_solver eauto using env_Forall2_wf, env_Forall2_fresh.
+  - induction Hp; rewrite /= ?later_and; auto using and_mono, later_intro.
+  - induction Hs; rewrite /= ?later_sep; auto using sep_mono, later_intro.
+Qed.
+
+Lemma tac_next Δ Δ' Q Q' :
+  StripLaterEnvs Δ Δ' → StripLaterL Q Q' → Δ' ⊢ Q' → Δ ⊢ Q.
+Proof. intros ?? HQ. by rewrite -(strip_later_l Q) strip_later_env_sound HQ. Qed.
+
+Lemma tac_löb Δ Δ' i Q :
+  envs_persistent Δ = true →
+  envs_app true (Esnoc Enil i (▷ Q)%I) Δ = Some Δ' →
+  Δ' ⊢ Q → Δ ⊢ Q.
+Proof.
+  intros ?? HQ. rewrite (persistentP Δ) envs_app_sound //; simpl.
+  rewrite right_id -{2}(always_elim Q) -(löb (□ Q)); apply impl_intro_l.
+  rewrite -always_later -{1}(always_always (□ (▷ Q))) always_and_sep_l'.
+  by rewrite -always_sep wand_elim_r HQ.
+Qed.
+
+(** * Always *)
+Lemma tac_always_intro Δ Q : envs_persistent Δ = true → Δ ⊢ Q → Δ ⊢ □ Q.
+Proof. intros. by apply: always_intro. Qed.
+
+Class ToPersistentP (P Q : uPred M) := to_persistentP : P ⊢ □ Q.
+Arguments to_persistentP : clear implicits.
+Global Instance to_persistentP_always_trans P Q :
+  ToPersistentP P Q → ToPersistentP (□ P) Q | 0.
+Proof. rewrite /ToPersistentP=> ->. by rewrite always_always. Qed.
+Global Instance to_persistentP_always P : ToPersistentP (□ P) P | 1.
+Proof. done. Qed.
+Global Instance to_persistentP_persistent P :
+  PersistentP P → ToPersistentP P P | 100.
+Proof. done. Qed.
+
+Lemma tac_persistent Δ Δ' i p P P' Q :
+  envs_lookup i Δ = Some (p, P)%I → ToPersistentP P P' →
+  envs_replace i p true (Esnoc Enil i P') Δ = Some Δ' →
+  Δ' ⊢ Q → Δ ⊢ Q.
+Proof.
+  intros ??? <-. rewrite envs_replace_sound //; simpl. destruct p.
+  - by rewrite right_id (to_persistentP P) always_always wand_elim_r.
+  - by rewrite right_id (to_persistentP P) wand_elim_r.
+Qed.
+
+(** * Implication and wand *)
+Lemma tac_impl_intro Δ Δ' i P Q :
+  envs_persistent Δ = true →
+  envs_app false (Esnoc Enil i P) Δ = Some Δ' →
+  Δ' ⊢ Q → Δ ⊢ (P → Q).
+Proof.
+  intros ?? HQ. rewrite (persistentP Δ) envs_app_sound //; simpl.
+  by rewrite right_id always_wand_impl always_elim HQ.
+Qed.
+Lemma tac_impl_intro_persistent Δ Δ' i P P' Q :
+  ToPersistentP P P' →
+  envs_app true (Esnoc Enil i P') Δ = Some Δ' →
+  Δ' ⊢ Q → Δ ⊢ (P → Q).
+Proof.
+  intros ?? HQ. rewrite envs_app_sound //; simpl. apply impl_intro_l.
+  by rewrite right_id {1}(to_persistentP P) always_and_sep_l wand_elim_r.
+Qed.
+Lemma tac_impl_intro_pure Δ P φ Q : ToPure P φ → (φ → Δ ⊢ Q) → Δ ⊢ (P → Q).
+Proof.
+  intros. by apply impl_intro_l; rewrite (to_pure P); apply const_elim_l.
+Qed.
+
+Lemma tac_wand_intro Δ Δ' i P Q :
+  envs_app false (Esnoc Enil i P) Δ = Some Δ' → Δ' ⊢ Q → Δ ⊢ (P -★ Q).
+Proof.
+  intros. rewrite envs_app_sound //; simpl.
+  rewrite right_id. by apply wand_mono.
+Qed.
+Lemma tac_wand_intro_persistent Δ Δ' i P P' Q :
+  ToPersistentP P P' →
+  envs_app true (Esnoc Enil i P') Δ = Some Δ' →
+  Δ' ⊢ Q → Δ ⊢ (P -★ Q).
+Proof.
+  intros. rewrite envs_app_sound //; simpl.
+  rewrite right_id. by apply wand_mono.
+Qed.
+Lemma tac_wand_intro_pure Δ P φ Q : ToPure P φ → (φ → Δ ⊢ Q) → Δ ⊢ (P -★ Q).
+Proof.
+  intros. by apply wand_intro_l; rewrite (to_pure P); apply const_elim_sep_l.
+Qed.
+
+Class ToWand (R P Q : uPred M) := to_wand : R ⊢ (P -★ Q).
+Arguments to_wand : clear implicits.
+Global Instance to_wand_wand P Q : ToWand (P -★ Q) P Q.
+Proof. done. Qed.
+Global Instance to_wand_impl P Q : ToWand (P → Q) P Q.
+Proof. apply impl_wand. Qed.
+Global Instance to_wand_iff_l P Q : ToWand (P ↔ Q) P Q.
+Proof. by apply and_elim_l', impl_wand. Qed.
+Global Instance to_wand_iff_r P Q : ToWand (P ↔ Q) Q P.
+Proof. apply and_elim_r', impl_wand. Qed.
+
+(* This is pretty much [tac_specialize_assert] with [js:=[j]] and [tac_exact],
+but it is doing some work to keep the order of hypotheses preserved. *)
+Lemma tac_specialize Δ Δ' Δ'' i p j q P1 P2 R Q :
+  envs_lookup_delete i Δ = Some (p, P1, Δ') →
+  envs_lookup j (if p then Δ else Δ') = Some (q, R)%I →
+  ToWand R P1 P2 →
+  match p with
+  | true  => envs_simple_replace j q (Esnoc Enil j P2) Δ
+  | false => envs_replace j q false (Esnoc Enil j P2) Δ'
+             (* remove [i] and make [j] spatial *)
+  end = Some Δ'' →
+  Δ'' ⊢ Q → Δ ⊢ Q.
+Proof.
+  intros [? ->]%envs_lookup_delete_Some ??? <-. destruct p.
+  - rewrite envs_lookup_persistent_sound // envs_simple_replace_sound //; simpl.
+    destruct q.
+    + by rewrite assoc (to_wand R) always_wand wand_elim_r right_id wand_elim_r.
+    + by rewrite assoc (to_wand R) always_elim wand_elim_r right_id wand_elim_r.
+  - rewrite envs_lookup_sound //; simpl.
+    rewrite envs_lookup_sound // (envs_replace_sound' _ Δ'') //; simpl.
+    destruct q.
+    + by rewrite right_id assoc (to_wand R) always_elim wand_elim_r wand_elim_r.
+    + by rewrite assoc (to_wand R) wand_elim_r right_id wand_elim_r.
+Qed.
+
+Lemma tac_specialize_assert Δ Δ' Δ1 Δ2' j q lr js P1 P2 R Q :
+  envs_lookup_delete j Δ = Some (q, R, Δ')%I →
+  ToWand R P1 P2 →
+  ('(Δ1,Δ2) ← envs_split lr js Δ';
+    Δ2' ← envs_app (envs_persistent Δ1 && q) (Esnoc Enil j P2) Δ2;
+    Some (Δ1,Δ2')) = Some (Δ1,Δ2') → (* does not preserve position of [j] *)
+  Δ1 ⊢ P1 → Δ2' ⊢ Q → Δ ⊢ Q.
+Proof.
+  intros [? ->]%envs_lookup_delete_Some ?? HP1 <-.
+  destruct (envs_split _ _ _) as [[? Δ2]|] eqn:?; simplify_eq/=;
+    destruct (envs_app _ _ _) eqn:?; simplify_eq/=.
+  rewrite envs_lookup_sound // envs_split_sound //.
+  rewrite (envs_app_sound Δ2) //; simpl.
+  destruct q, (envs_persistent Δ1) eqn:?; simplify_eq/=.
+  - rewrite right_id (to_wand R) (persistentP Δ1) HP1.
+    by rewrite assoc -always_sep wand_elim_l wand_elim_r.
+  - by rewrite right_id (to_wand R) always_elim assoc HP1 wand_elim_l wand_elim_r.
+  - by rewrite right_id (to_wand R) assoc HP1 wand_elim_l wand_elim_r.
+  - by rewrite right_id (to_wand R) assoc HP1 wand_elim_l wand_elim_r. 
+Qed.
+
+Lemma tac_specialize_range_persistent Δ Δ' Δ'' j q P1 P2 R Q :
+  envs_lookup_delete j Δ = Some (q, R, Δ')%I →
+  ToWand R P1 P2 → PersistentP P1 →
+  envs_simple_replace j q (Esnoc Enil j P2) Δ = Some Δ'' →
+  Δ' ⊢ P1 → Δ'' ⊢ Q → Δ ⊢ Q.
+Proof.
+  intros [? ->]%envs_lookup_delete_Some ??? HP1 <-.
+  rewrite envs_lookup_sound //.
+  rewrite -(idemp uPred_and (envs_delete _ _ _)).
+  rewrite {1}HP1 (persistentP P1) always_and_sep_l assoc.
+  rewrite envs_simple_replace_sound' //; simpl. destruct q.
+  - by rewrite right_id (to_wand R) -always_sep wand_elim_l wand_elim_r.
+  - by rewrite right_id (to_wand R) always_elim wand_elim_l wand_elim_r.
+Qed.
+
+Lemma tac_specialize_domain_persistent Δ Δ' Δ'' j q P1 P2 P2' R Q :
+  envs_lookup_delete j Δ = Some (q, R, Δ')%I →
+  ToWand R P1 P2 → ToPersistentP P2 P2' →
+  envs_replace j q true (Esnoc Enil j P2') Δ = Some Δ'' →
+  Δ' ⊢ P1 → Δ'' ⊢ Q → Δ ⊢ Q.
+Proof.
+  intros [? ->]%envs_lookup_delete_Some ??? HP1 <-.
+  rewrite -(idemp uPred_and Δ) {1}envs_lookup_sound //; simpl; rewrite HP1.
+  rewrite envs_replace_sound //; simpl.
+  rewrite (sep_elim_r _ (_ -★ _)) right_id. destruct q.
+  - rewrite (to_wand R) always_elim wand_elim_l.
+    by rewrite (to_persistentP P2) always_and_sep_l' wand_elim_r.
+  - rewrite (to_wand R) wand_elim_l.
+    by rewrite (to_persistentP P2) always_and_sep_l' wand_elim_r.
+Qed.
+
+Lemma tac_revert Δ Δ' i p P Q :
+  envs_lookup_delete i Δ = Some (p,P,Δ') →
+  Δ' ⊢ (if p then □ P → Q else P -★ Q) → Δ ⊢ Q.
+Proof.
+  intros ? HQ. rewrite envs_lookup_delete_sound //; simpl. destruct p.
+  - by rewrite HQ -always_and_sep_l impl_elim_r.
+  - by rewrite HQ wand_elim_r.
+Qed.
+
+Lemma tac_assert Δ Δ1 Δ2 Δ2' lr js j P Q :
+  envs_split lr js Δ = Some (Δ1,Δ2) →
+  envs_app (envs_persistent Δ1) (Esnoc Enil j P) Δ2 = Some Δ2' →
+  Δ1 ⊢ P → Δ2' ⊢ Q → Δ ⊢ Q.
+Proof.
+  intros ?? HP ?. rewrite envs_split_sound //.
+  destruct (envs_persistent Δ1) eqn:?.
+  - rewrite (persistentP Δ1) HP envs_app_sound //; simpl.
+    by rewrite right_id wand_elim_r.
+  - rewrite HP envs_app_sound //; simpl. by rewrite right_id wand_elim_r.
+Qed.
+
+Lemma tac_assert_persistent Δ Δ' j P Q :
+  PersistentP P →
+  envs_app true (Esnoc Enil j P) Δ = Some Δ' →
+  Δ ⊢ P → Δ' ⊢ Q → Δ ⊢ Q.
+Proof.
+  intros ?? HP ?.
+  rewrite -(idemp uPred_and Δ) {1}HP envs_app_sound //; simpl.
+  by rewrite right_id {1}(persistentP P) always_and_sep_l wand_elim_r.
+Qed.
+
+Lemma tac_pose_proof Δ Δ' j P Q :
+  True ⊢ P → envs_app true (Esnoc Enil j P) Δ = Some Δ' →
+  Δ' ⊢ Q → Δ ⊢ Q.
+Proof.
+  intros HP ? <-. rewrite envs_app_sound //; simpl.
+  by rewrite -HP left_id always_const wand_True.
+Qed.
+
+Lemma tac_apply Δ Δ' i p R P1 P2 :
+  envs_lookup_delete i Δ = Some (p, R, Δ')%I → ToWand R P1 P2 →
+  Δ' ⊢ P1 → Δ ⊢ P2.
+Proof.
+  intros ?? HP1. rewrite envs_lookup_delete_sound' //.
+  by rewrite (to_wand R) HP1 wand_elim_l.
+Qed.
+
+(** * Rewriting *)
+Lemma tac_rewrite Δ i p Pxy (lr : bool) Q :
+  envs_lookup i Δ = Some (p, Pxy) →
+  ∀ {A : cofeT} x y (Φ : A → uPred M),
+    Pxy ⊢ (x ≡ y)%I →
+    Q ⊣⊢ Φ (if lr then y else x) →
+    (∀ n, Proper (dist n ==> dist n) Φ) →
+    Δ ⊢ Φ (if lr then x else y) → Δ ⊢ Q.
+Proof.
+  intros ? A x y ? HPxy -> ?; apply eq_rewrite; auto.
+  rewrite {1}envs_lookup_sound' //; rewrite sep_elim_l HPxy.
+  destruct lr; auto using eq_sym.
+Qed.
+
+Lemma tac_rewrite_in Δ i p Pxy j q P (lr : bool) Q :
+  envs_lookup i Δ = Some (p, Pxy) →
+  envs_lookup j Δ = Some (q, P)%I →
+  ∀ {A : cofeT} Δ' x y (Φ : A → uPred M),
+    Pxy ⊢ (x ≡ y)%I →
+    P ⊣⊢ Φ (if lr then y else x) →
+    (∀ n, Proper (dist n ==> dist n) Φ) →
+    envs_simple_replace j q (Esnoc Enil j (Φ (if lr then x else y))) Δ = Some Δ' →
+    Δ' ⊢ Q → Δ ⊢ Q.
+Proof.
+  intros ?? A Δ' x y Φ HPxy HP ?? <-.
+  rewrite -(idemp uPred_and Δ) {2}(envs_lookup_sound' _ i) //.
+  rewrite sep_elim_l HPxy always_and_sep_r.
+  rewrite (envs_simple_replace_sound _ _ j) //; simpl. destruct q.
+  - rewrite HP right_id -assoc; apply wand_elim_r'. destruct lr.
+    + apply (eq_rewrite x y (λ y, □ Φ y -★ Δ')%I); eauto with I. solve_proper.
+    + apply (eq_rewrite y x (λ y, □ Φ y -★ Δ')%I); eauto using eq_sym with I.
+      solve_proper.
+  - rewrite HP right_id -assoc; apply wand_elim_r'. destruct lr.
+    + apply (eq_rewrite x y (λ y, Φ y -★ Δ')%I); eauto with I. solve_proper.
+    + apply (eq_rewrite y x (λ y, Φ y -★ Δ')%I); eauto using eq_sym with I.
+      solve_proper.
+Qed.
+
+(** * Conjunction splitting *)
+Class AndSplit (P Q1 Q2 : uPred M) := and_split : (Q1 ∧ Q2) ⊢ P.
+Arguments and_split : clear implicits.
+
+Global Instance and_split_and P1 P2 : AndSplit (P1 ∧ P2) P1 P2.
+Proof. done. Qed.
+Global Instance and_split_sep_persistent_l P1 P2 :
+  PersistentP P1 → AndSplit (P1 ★ P2) P1 P2.
+Proof. intros. by rewrite /AndSplit always_and_sep_l. Qed.
+Global Instance and_split_sep_persistent_r P1 P2 :
+  PersistentP P2 → AndSplit (P1 ★ P2) P1 P2.
+Proof. intros. by rewrite /AndSplit always_and_sep_r. Qed.
+
+Lemma tac_and_split Δ P Q1 Q2 : AndSplit P Q1 Q2 → Δ ⊢ Q1 → Δ ⊢ Q2 → Δ ⊢ P.
+Proof. intros. rewrite -(and_split P). by apply and_intro. Qed.
+
+(** * Separating conjunction splitting *)
+Class SepSplit (P Q1 Q2 : uPred M) := sep_split : (Q1 ★ Q2) ⊢ P.
+Arguments sep_split : clear implicits.
+
+Global Instance sep_split_sep P1 P2 : SepSplit (P1 ★ P2) P1 P2 | 100.
+Proof. done. Qed.
+Global Instance sep_split_ownM (a b : M) :
+  SepSplit (uPred_ownM (a ⋅ b)) (uPred_ownM a) (uPred_ownM b) | 99.
+Proof. by rewrite /SepSplit ownM_op. Qed.
+
+Lemma tac_sep_split Δ Δ1 Δ2 lr js P Q1 Q2 :
+  SepSplit P Q1 Q2 →
+  envs_split lr js Δ = Some (Δ1,Δ2) →
+  Δ1 ⊢ Q1 → Δ2 ⊢ Q2 → Δ ⊢ P.
+Proof.
+  intros. rewrite envs_split_sound // -(sep_split P). by apply sep_mono.
+Qed.
+
+(** * Combining *)
+Lemma tac_combine Δ1 Δ2 Δ3 Δ4 i1 p P1 i2 q P2 j P Q :
+  envs_lookup_delete i1 Δ1 = Some (p,P1,Δ2) →
+  envs_lookup_delete i2 (if p then Δ1 else Δ2) = Some (q,P2,Δ3) →
+  SepSplit P P1 P2 →
+  envs_app (p && q) (Esnoc Enil j P)
+    (if q then (if p then Δ1 else Δ2) else Δ3) = Some Δ4 →
+  Δ4 ⊢ Q → Δ1 ⊢ Q.
+Proof.
+  intros [? ->]%envs_lookup_delete_Some [? ->]%envs_lookup_delete_Some ?? <-.
+  destruct p.
+  - rewrite envs_lookup_persistent_sound //. destruct q.
+    + rewrite envs_lookup_persistent_sound // envs_app_sound //; simpl.
+      by rewrite right_id assoc -always_sep (sep_split P) wand_elim_r.
+    + rewrite envs_lookup_sound // envs_app_sound //; simpl.
+      by rewrite right_id assoc always_elim (sep_split P) wand_elim_r.
+  - rewrite envs_lookup_sound //; simpl. destruct q.
+    + rewrite envs_lookup_persistent_sound // envs_app_sound //; simpl.
+      by rewrite right_id assoc always_elim (sep_split P) wand_elim_r.
+    + rewrite envs_lookup_sound // envs_app_sound //; simpl.
+      by rewrite right_id assoc (sep_split P) wand_elim_r.
+Qed.
+
+(** * Conjunction/separating conjunction elimination *)
+Class SepDestruct (p : bool) (P Q1 Q2 : uPred M) :=
+  sep_destruct : if p then □ P ⊢ □ (Q1 ∧ Q2) else P ⊢ (Q1 ★ Q2).
+Arguments sep_destruct : clear implicits.
+Lemma sep_destruct_spatial p P Q1 Q2 : P ⊢ (Q1 ★ Q2) → SepDestruct p P Q1 Q2.
+Proof. destruct p; simpl=>->; by rewrite ?sep_and. Qed.
+
+Global Instance sep_destruct_sep p P Q : SepDestruct p (P ★ Q) P Q.
+Proof. by apply sep_destruct_spatial. Qed.
+Global Instance sep_destruct_ownM p (a b : M) :
+  SepDestruct p (uPred_ownM (a ⋅ b)) (uPred_ownM a) (uPred_ownM b).
+Proof. apply sep_destruct_spatial. by rewrite ownM_op. Qed.
+
+Global Instance sep_destruct_and P Q : SepDestruct true (P ∧ Q) P Q.
+Proof. done. Qed.
+Global Instance sep_destruct_and_persistent_l P Q :
+  PersistentP P → SepDestruct false (P ∧ Q) P Q.
+Proof. intros; red. by rewrite always_and_sep_l. Qed.
+Global Instance sep_destruct_and_persistent_r P Q :
+  PersistentP Q → SepDestruct false (P ∧ Q) P Q.
+Proof. intros; red. by rewrite always_and_sep_r. Qed.
+
+Global Instance sep_destruct_later p P Q1 Q2 :
+  SepDestruct p P Q1 Q2 → SepDestruct p (▷ P) (▷ Q1) (▷ Q2).
+Proof.
+  destruct p=> /= HP.
+  - by rewrite -later_and !always_later HP.
+  - by rewrite -later_sep HP.
+Qed.
+
+Lemma tac_sep_destruct Δ Δ' i p j1 j2 P P1 P2 Q :
+  envs_lookup i Δ = Some (p, P)%I → SepDestruct p P P1 P2 →
+  envs_simple_replace i p (Esnoc (Esnoc Enil j1 P1) j2 P2) Δ = Some Δ' →
+  Δ' ⊢ Q → Δ ⊢ Q.
+Proof.
+  intros. rewrite envs_simple_replace_sound //; simpl. destruct p.
+  - by rewrite (sep_destruct true P) right_id (comm uPred_and) wand_elim_r.
+  - by rewrite (sep_destruct false P) right_id (comm uPred_sep P1) wand_elim_r.
+Qed.
+
+(** * Framing *)
+Class Frame (R P Q : uPred M) := frame : (R ★ Q) ⊢ P.
+Arguments frame : clear implicits.
+
+Global Instance frame_here R : Frame R R True | 1.
+Proof. by rewrite /Frame right_id. Qed.
+Global Instance frame_here_l R P : Frame R (R ★ P) P | 0.
+Proof. done. Qed.
+Global Instance frame_here_r R P : Frame R (P ★ R) P | 0.
+Proof. by rewrite /Frame comm. Qed.
+Global Instance frame_here_and_l R P : Frame R (R ∧ P) P | 0.
+Proof. by rewrite /Frame sep_and. Qed.
+Global Instance frame_here_and_r R P : Frame R (P ∧ R) P | 0.
+Proof. by rewrite /Frame sep_and comm. Qed.
+Global Instance frame_sep_l R P1 P2 Q :
+  Frame R P1 Q → Frame R (P1 ★ P2) (Q ★ P2).
+Proof. rewrite /Frame => <-. solve_sep_entails. Qed.
+Global Instance frame_sep_r R P1 P2 Q :
+  Frame R P2 Q → Frame R (P1 ★ P2) (P1 ★ Q).
+Proof. rewrite /Frame => <-. solve_sep_entails. Qed.
+Global Instance frame_or R P1 P2 Q1 Q2 :
+  Frame R P1 Q1 → Frame R P2 Q2 → Frame R (P1 ∨ P2) (Q1 ∨ Q2).
+Proof. rewrite /Frame=> <- <-. by rewrite -sep_or_l. Qed.
+Global Instance frame_exist {A} R (Φ Ψ : A → uPred M) :
+  (∀ a, Frame R (Φ a) (Ψ a)) → Frame R (∃ x, Φ x) (∃ x, Ψ x).
+Proof. rewrite /Frame=> ?. by rewrite sep_exist_l; apply exist_mono. Qed.
+Global Instance frame_forall {A} R (Φ Ψ : A → uPred M) :
+  (∀ a, Frame R (Φ a) (Ψ a)) → Frame R (∀ x, Φ x) (∀ x, Ψ x).
+Proof. rewrite /Frame=> ?. by rewrite sep_forall_l; apply forall_mono. Qed.
+
+Lemma tac_frame Δ Δ' i p R P Q :
+  envs_lookup_delete i Δ = Some (p, R, Δ')%I → Frame R P Q →
+  (if p then Δ else Δ') ⊢ Q → Δ ⊢ P.
+Proof.
+  intros [? ->]%envs_lookup_delete_Some ? HQ; destruct p.
+  - by rewrite envs_lookup_persistent_sound // HQ always_elim.
+  - rewrite envs_lookup_sound //; simpl. by rewrite HQ.
+Qed.
+
+(** * Disjunction *)
+Class OrSplit (P Q1 Q2 : uPred M) := or_split : (Q1 ∨ Q2) ⊢ P.
+Arguments or_split : clear implicits.
+Global Instance or_split_or P1 P2 : OrSplit (P1 ∨ P2) P1 P2.
+Proof. done. Qed.
+
+Lemma tac_or_l Δ P Q1 Q2 : OrSplit P Q1 Q2 → Δ ⊢ Q1 → Δ ⊢ P.
+Proof. intros. rewrite -(or_split P). by apply or_intro_l'. Qed.
+Lemma tac_or_r Δ P Q1 Q2 : OrSplit P Q1 Q2 → Δ ⊢ Q2 → Δ ⊢ P.
+Proof. intros. rewrite -(or_split P). by apply or_intro_r'. Qed.
+
+Class OrDestruct P Q1 Q2 := or_destruct : P ⊢ (Q1 ∨ Q2).
+Arguments or_destruct : clear implicits.
+Global Instance or_destruct_or P Q : OrDestruct (P ∨ Q) P Q.
+Proof. done. Qed.
+Global Instance or_destruct_later P Q1 Q2 :
+  OrDestruct P Q1 Q2 → OrDestruct (▷ P) (▷ Q1) (▷ Q2).
+Proof. rewrite /OrDestruct=>->. by rewrite later_or. Qed.
+
+Lemma tac_or_destruct Δ Δ1 Δ2 i p j1 j2 P P1 P2 Q :
+  envs_lookup i Δ = Some (p, P)%I → OrDestruct P P1 P2 →
+  envs_simple_replace i p (Esnoc Enil j1 P1) Δ = Some Δ1 →
+  envs_simple_replace i p (Esnoc Enil j2 P2) Δ = Some Δ2 →
+  Δ1 ⊢ Q → Δ2 ⊢ Q → Δ ⊢ Q.
+Proof.
+  intros ???? HP1 HP2. rewrite envs_lookup_sound //. destruct p.
+  - rewrite (or_destruct P) always_or sep_or_r; apply or_elim. simpl.
+    + rewrite (envs_simple_replace_sound' _ Δ1) //.
+      by rewrite /= right_id wand_elim_r.
+    + rewrite (envs_simple_replace_sound' _ Δ2) //.
+      by rewrite /= right_id wand_elim_r.
+  - rewrite (or_destruct P) sep_or_r; apply or_elim.
+    + rewrite (envs_simple_replace_sound' _ Δ1) //.
+      by rewrite /= right_id wand_elim_r.
+    + rewrite (envs_simple_replace_sound' _ Δ2) //.
+      by rewrite /= right_id wand_elim_r.
+Qed.
+
+(** * Forall *)
+Lemma tac_forall_intro {A} Δ (Φ : A → uPred M) : (∀ a, Δ ⊢ Φ a) → Δ ⊢ (∀ a, Φ a).
+Proof. apply forall_intro. Qed.
+
+Lemma tac_forall_specialize {A} Δ Δ' i p (Φ : A → uPred M) Q a :
+  envs_lookup i Δ = Some (p, ∀ a, Φ a)%I →
+  envs_simple_replace i p (Esnoc Enil i (Φ a)) Δ = Some Δ' →
+  Δ' ⊢ Q → Δ ⊢ Q.
+Proof.
+  intros. rewrite envs_simple_replace_sound //; simpl.
+  destruct p; by rewrite /= right_id (forall_elim a) wand_elim_r.
+Qed.
+
+Lemma tac_forall_revert {A} Δ (Φ : A → uPred M) :
+  Δ ⊢ (∀ a, Φ a) → (∀ a, Δ ⊢ Φ a).
+Proof. intros HΔ a. by rewrite HΔ (forall_elim a). Qed.
+
+(** * Existential *)
+Class ExistSplit {A} (P : uPred M) (Φ : A → uPred M) :=
+  exist_split : (∃ x, Φ x) ⊢ P.
+Arguments exist_split {_} _ _ {_}.
+Global Instance exist_split_exist {A} (Φ: A → uPred M): ExistSplit (∃ a, Φ a) Φ.
+Proof. done. Qed.
+
+Lemma tac_exist {A} Δ P (Φ : A → uPred M) a : ExistSplit P Φ → Δ ⊢ Φ a → Δ ⊢ P.
+Proof. intros. rewrite -(exist_split P). eauto using exist_intro'. Qed.
+
+Class ExistDestruct {A} (P : uPred M) (Φ : A → uPred M) :=
+  exist_destruct : P ⊢ (∃ x, Φ x).
+Arguments exist_destruct {_} _ _ {_}.
+Global Instance exist_destruct_exist {A} (Φ : A → uPred M) :
+  ExistDestruct (∃ a, Φ a) Φ.
+Proof. done. Qed.
+Global Instance exist_destruct_later {A} P (Φ : A → uPred M) :
+  Inhabited A → ExistDestruct P Φ → ExistDestruct (▷ P) (λ a, ▷ (Φ a))%I.
+Proof. rewrite /ExistDestruct=> ? ->. by rewrite later_exist. Qed.
+
+Lemma tac_exist_destruct {A} Δ i p j P (Φ : A → uPred M) Q :
+  envs_lookup i Δ = Some (p, P)%I → ExistDestruct P Φ →
+  (∀ a, ∃ Δ',
+    envs_simple_replace i p (Esnoc Enil j (Φ a)) Δ = Some Δ' ∧ Δ' ⊢ Q) →
+  Δ ⊢ Q.
+Proof.
+  intros ?? HΦ. rewrite envs_lookup_sound //. destruct p.
+  - rewrite (exist_destruct P) always_exist sep_exist_r.
+    apply exist_elim=> a; destruct (HΦ a) as (Δ'&?&?).
+    rewrite envs_simple_replace_sound' //; simpl.
+    by rewrite right_id wand_elim_r.
+  - rewrite (exist_destruct P) sep_exist_r.
+    apply exist_elim=> a; destruct (HΦ a) as (Δ'&?&?).
+    rewrite envs_simple_replace_sound' //; simpl.
+    by rewrite right_id wand_elim_r.
+Qed.
+End tactics.
