proofmode/ghost_ownership.v
@@ -1,0 +1,15 @@
+From iris.proofmode Require Import coq_tactics.
+From iris.proofmode Require Export tactics.
+From iris.program_logic Require Export ghost_ownership.
+
+Section ghost.
+Context `{inG Λ Σ A}.
+Implicit Types a b : A.
+
+Global Instance sep_destruct_own p γ a b :
+  SepDestruct p (own γ (a ⋅ b)) (own γ a) (own γ b).
+Proof. apply sep_destruct_spatial. by rewrite own_op. Qed.
+Global Instance sep_split_own γ a b :
+  SepSplit (own γ (a ⋅ b)) (own γ a) (own γ b) | 90.
+Proof. by rewrite /SepSplit own_op. Qed.
+End ghost.
