proofmode/notation.v
@@ -1,0 +1,27 @@
+From iris.proofmode Require Import coq_tactics environments.
+From iris.prelude Require Export strings.
+
+Delimit Scope proof_scope with env.
+Arguments Envs _ _%proof_scope _%proof_scope.
+Arguments Enil {_}.
+Arguments Esnoc {_} _%proof_scope _%string _%uPred_scope.
+
+Notation "​" := Enil (format "​") : proof_scope.
+Notation "​ Γ H : P" := (Esnoc Γ H P)
+  (at level 1, P at level 200,
+   left associativity, format "​ Γ H  :  P '//'") : proof_scope.
+Notation "Γ '--------------------------------------' □ Δ '--------------------------------------' ★ Q" :=
+  (of_envs (Envs Γ Δ) ⊢ Q%I)
+  (at level 1, Q at level 200, left associativity,
+  format "Γ '--------------------------------------' □ '//' Δ '--------------------------------------' ★ '//' Q '//'") :
+  C_scope.
+Notation "Δ '--------------------------------------' ★ Q" :=
+  (of_envs (Envs Enil Δ) ⊢ Q%I)
+  (at level 1, Q at level 200, left associativity,
+  format "Δ '--------------------------------------' ★ '//' Q '//'") : C_scope.
+Notation "Γ '--------------------------------------' □ Q" :=
+  (of_envs (Envs Γ Enil) ⊢ Q%I)
+  (at level 1, Q at level 200, left associativity,
+  format "Γ '--------------------------------------' □ '//' Q '//'")  : C_scope.
+Notation "​​ Q" := (of_envs (Envs Enil Enil) ⊢ Q%I)
+  (at level 1, format "​​ Q") : C_scope.
