proofmode/pviewshifts.v
@@ -1,0 +1,235 @@
+From iris.proofmode Require Import coq_tactics spec_patterns.
+From iris.proofmode Require Export tactics.
+From iris.program_logic Require Export pviewshifts.
+Import uPred.
+
+Section pvs.
+Context {Λ : language} {Σ : iFunctor}.
+Implicit Types P Q : iProp Λ Σ.
+
+Global Instance sep_split_pvs E P Q1 Q2 :
+  SepSplit P Q1 Q2 → SepSplit (|={E}=> P) (|={E}=> Q1) (|={E}=> Q2).
+Proof. rewrite /SepSplit=><-. apply pvs_sep. Qed.
+Global Instance or_split_pvs E1 E2 P Q1 Q2 :
+  OrSplit P Q1 Q2 → OrSplit (|={E1,E2}=> P) (|={E1,E2}=> Q1) (|={E1,E2}=> Q2).
+Proof. rewrite /OrSplit=><-. apply or_elim; apply pvs_mono; auto with I. Qed.
+Global Instance exists_split_pvs {A} E1 E2 P (Φ : A → iProp Λ Σ) :
+  ExistSplit P Φ → ExistSplit (|={E1,E2}=> P) (λ a, |={E1,E2}=> Φ a)%I.
+Proof.
+  rewrite /ExistSplit=><-. apply exist_elim=> a. by rewrite -(exist_intro a).
+Qed.
+Global Instance frame_pvs E1 E2 R P Q :
+  Frame R P Q → Frame R (|={E1,E2}=> P) (|={E1,E2}=> Q).
+Proof. rewrite /Frame=><-. by rewrite pvs_frame_l. Qed.
+Global Instance to_wand_pvs E1 E2 R P Q :
+  ToWand R P Q → ToWand R (|={E1,E2}=> P) (|={E1,E2}=> Q).
+Proof. rewrite /ToWand=>->. apply wand_intro_l. by rewrite pvs_wand_r. Qed.
+
+Class FSASplit {A} (P : iProp Λ Σ) (E : coPset)
+    (fsa : FSA Λ Σ A) (fsaV : Prop) (Φ : A → iProp Λ Σ) := {
+  fsa_split : fsa E Φ ⊢ P;
+  fsa_split_fsa :> FrameShiftAssertion fsaV fsa;
+}.
+Global Arguments fsa_split {_} _ _ _ _ _ {_}.
+Global Instance fsa_split_pvs E P :
+  FSASplit (|={E}=> P)%I E pvs_fsa True (λ _, P).
+Proof. split. done. apply _. Qed.
+
+Lemma tac_pvs_intro Δ E Q : Δ ⊢ Q → Δ ⊢ |={E}=> Q.
+Proof. intros ->. apply pvs_intro. Qed.
+
+Lemma tac_pvs_elim Δ Δ' E1 E2 E3 i p P Q :
+  envs_lookup i Δ = Some (p, |={E1,E2}=> P)%I →
+  envs_replace i p false (Esnoc Enil i P) Δ = Some Δ' →
+  E2 ⊆ E1 ∪ E3 →
+  Δ' ⊢ (|={E2,E3}=> Q) → Δ ⊢ |={E1,E3}=> Q.
+Proof.
+  intros ??? HQ. rewrite envs_replace_sound //; simpl. destruct p.
+  - by rewrite always_elim right_id pvs_frame_r wand_elim_r HQ pvs_trans.
+  - by rewrite right_id pvs_frame_r wand_elim_r HQ pvs_trans.
+Qed.
+
+Lemma tac_pvs_elim_fsa {A} (fsa : FSA Λ Σ A) fsaV Δ Δ' E i p P Q Φ :
+  envs_lookup i Δ = Some (p, |={E}=> P)%I → FSASplit Q E fsa fsaV Φ →
+  envs_replace i p false (Esnoc Enil i P) Δ = Some Δ' →
+  Δ' ⊢ fsa E Φ → Δ ⊢ Q.
+Proof.
+  intros ???. rewrite -(fsa_split Q) -fsa_pvs_fsa.
+  eapply tac_pvs_elim; set_solver.
+Qed.
+
+Lemma tac_pvs_timeless Δ Δ' E1 E2 i p P Q :
+  envs_lookup i Δ = Some (p, ▷ P)%I → TimelessP P →
+  envs_simple_replace i p (Esnoc Enil i P) Δ = Some Δ' →
+  Δ' ⊢ (|={E1,E2}=> Q) → Δ ⊢ (|={E1,E2}=> Q).
+Proof.
+  intros ??? HQ. rewrite envs_simple_replace_sound //; simpl.
+  destruct p.
+  - rewrite always_later (pvs_timeless E1 (□ P)%I) pvs_frame_r.
+    by rewrite right_id wand_elim_r HQ pvs_trans; last set_solver.
+  - rewrite (pvs_timeless E1 P) pvs_frame_r right_id wand_elim_r HQ.
+    by rewrite pvs_trans; last set_solver.
+Qed.
+
+Lemma tac_pvs_timeless_fsa {A} (fsa : FSA Λ Σ A) fsaV Δ Δ' E i p P Q Φ :
+  FSASplit Q E fsa fsaV Φ →
+  envs_lookup i Δ = Some (p, ▷ P)%I → TimelessP P →
+  envs_simple_replace i p (Esnoc Enil i P) Δ = Some Δ' →
+  Δ' ⊢ fsa E Φ → Δ ⊢ Q.
+Proof.
+  intros ????. rewrite -(fsa_split Q) -fsa_pvs_fsa.
+  eauto using tac_pvs_timeless.
+Qed.
+
+Hint Immediate env_special_nil_persistent : typeclass_instances.
+Lemma tac_pvs_assert {A} (fsa : FSA Λ Σ A) fsaV Δ Δ1 Δ2 Δ2' E lr js j P Q Φ :
+  FSASplit Q E fsa fsaV Φ →
+  envs_split lr js Δ = Some (Δ1,Δ2) →
+  envs_app false (Esnoc Enil j P) Δ2 = Some Δ2' →
+  Δ1 ⊢ (|={E}=> P) → Δ2' ⊢ fsa E Φ → Δ ⊢ Q.
+Proof.
+  intros ??? HP HQ. rewrite -(fsa_split Q) -fsa_pvs_fsa -HQ envs_split_sound //.
+  rewrite HP envs_app_sound //; simpl.
+  by rewrite right_id pvs_frame_r wand_elim_r.
+Qed.
+End pvs.
+
+Tactic Notation "iPvsIntro" := apply tac_pvs_intro.
+
+Tactic Notation "iPvsCore" constr(H) :=
+  match goal with
+  | |- _ ⊢ |={_,_}=> _ =>
+    eapply tac_pvs_elim with _ _ H _ _;
+      [env_cbv; reflexivity || fail "iPvs:" H "not found"
+      |env_cbv; reflexivity
+      |try (rewrite (idemp_L (∪)); reflexivity)|]
+  | |- _ =>
+    eapply tac_pvs_elim_fsa with _ _ _ _ H _ _ _;
+      [env_cbv; reflexivity || fail "iPvs:" H "not found"
+      |let P := match goal with |- FSASplit ?P _ _ _ _ => P end in
+       apply _ || fail "iPvs: " P "not a pvs"
+      |env_cbv; reflexivity|simpl]
+  end.
+
+Tactic Notation "iPvs" open_constr(H) :=
+  iPoseProof H as (fun H => iPvsCore H; last iDestructHyp H as "?").
+Tactic Notation "iPvs" open_constr(H) "as" constr(pat) :=
+  iPoseProof H as (fun H => iPvsCore H; last iDestructHyp H as pat).
+Tactic Notation "iPvs" open_constr(H) "as" "{" simple_intropattern(x1) "}"
+    constr(pat) :=
+  iPoseProof H as (fun H => iPvsCore H; last iDestructHyp H as { x1 } pat).
+Tactic Notation "iPvs" open_constr(H) "as" "{" simple_intropattern(x1)
+    simple_intropattern(x2) "}" constr(pat) :=
+  iPoseProof H as (fun H => iPvsCore H; last iDestructHyp H as { x1 x2 } pat).
+Tactic Notation "iPvs" open_constr(H) "as" "{" simple_intropattern(x1)
+    simple_intropattern(x2) simple_intropattern(x3) "}" constr(pat) :=
+  iPoseProof H as (fun H => iPvsCore H; last iDestructHyp H as { x1 x2 x3 } pat).
+Tactic Notation "iPvs" open_constr(H) "as" "{" simple_intropattern(x1)
+    simple_intropattern(x2) simple_intropattern(x3) simple_intropattern(x4) "}"
+    constr(pat) :=
+  iPoseProof H as (fun H =>
+    iPvsCore H; last iDestructHyp H as { x1 x2 x3 x4 } pat).
+Tactic Notation "iPvs" open_constr(H) "as" "{" simple_intropattern(x1)
+    simple_intropattern(x2) simple_intropattern(x3) simple_intropattern(x4)
+    simple_intropattern(x5) "}" constr(pat) :=
+  iPoseProof H as (fun H =>
+    iPvsCore H; last iDestructHyp H as { x1 x2 x3 x4 x5 } pat).
+Tactic Notation "iPvs" open_constr(H) "as" "{" simple_intropattern(x1)
+    simple_intropattern(x2) simple_intropattern(x3) simple_intropattern(x4)
+    simple_intropattern(x5) simple_intropattern(x6) "}" constr(pat) :=
+  iPoseProof H as (fun H =>
+    iPvsCore H; last iDestructHyp H as { x1 x2 x3 x4 x5 x6 } pat).
+Tactic Notation "iPvs" open_constr(H) "as" "{" simple_intropattern(x1)
+    simple_intropattern(x2) simple_intropattern(x3) simple_intropattern(x4)
+    simple_intropattern(x5) simple_intropattern(x6) simple_intropattern(x7) "}"
+    constr(pat) :=
+  iPoseProof H as (fun H =>
+    iPvsCore H; last iDestructHyp H as { x1 x2 x3 x4 x5 x6 x7 } pat).
+Tactic Notation "iPvs" open_constr(H) "as" "{" simple_intropattern(x1)
+    simple_intropattern(x2) simple_intropattern(x3) simple_intropattern(x4)
+    simple_intropattern(x5) simple_intropattern(x6) simple_intropattern(x7)
+    simple_intropattern(x8) "}" constr(pat) :=
+  iPoseProof H as (fun H =>
+    iPvsCore H; last iDestructHyp H as { x1 x2 x3 x4 x5 x6 x7 x8 } pat).
+
+Tactic Notation "iPvs" open_constr(lem) constr(Hs) :=
+  iPoseProof lem Hs as (fun H => iPvsCore H; last iDestructHyp H as "?").
+Tactic Notation "iPvs" open_constr(lem) constr(Hs) "as" constr(pat) :=
+  iPoseProof lem Hs as (fun H => iPvsCore H; last iDestructHyp H as pat).
+Tactic Notation "iPvs" open_constr(lem) constr(Hs) "as" "{"
+    simple_intropattern(x1) "}" constr(pat) :=
+  iPoseProof lem Hs as (fun H => iPvsCore H; last iDestructHyp H as { x1 } pat).
+Tactic Notation "iPvs" open_constr(lem) constr(Hs) "as" "{"
+    simple_intropattern(x1) simple_intropattern(x2) "}" constr(pat) :=
+  iPoseProof lem Hs as (fun H =>
+    iPvsCore H; last iDestructHyp H as { x1 x2 } pat).
+Tactic Notation "iPvs" open_constr(lem) constr(Hs) "as" "{"
+    simple_intropattern(x1) simple_intropattern(x2) simple_intropattern(x3) "}"
+    constr(pat) :=
+  iPoseProof lem Hs as (fun H =>
+    iPvsCore H; last iDestructHyp H as { x1 x2 x3 } pat).
+Tactic Notation "iPvs" open_constr(lem) constr(Hs) "as" "{"
+    simple_intropattern(x1) simple_intropattern(x2) simple_intropattern(x3)
+    simple_intropattern(x4) "}" constr(pat) :=
+  iPoseProof lem Hs as (fun H =>
+    iPvsCore H; last iDestructHyp H as { x1 x2 x3 x4 } pat).
+Tactic Notation "iPvs" open_constr(lem) constr(Hs) "as" "{"
+    simple_intropattern(x1) simple_intropattern(x2) simple_intropattern(x3)
+    simple_intropattern(x4) simple_intropattern(x5) "}" constr(pat) :=
+  iPoseProof lem Hs as (fun H =>
+    iPvsCore H; last iDestructHyp H as { x1 x2 x3 x4 x5 } pat).
+Tactic Notation "iPvs" open_constr(lem) constr(Hs) "as" "{"
+    simple_intropattern(x1) simple_intropattern(x2) simple_intropattern(x3)
+    simple_intropattern(x4) simple_intropattern(x5) simple_intropattern(x6) "}"
+    constr(pat) :=
+  iPoseProof lem Hs as (fun H =>
+    iPvsCore H; last iDestructHyp H as { x1 x2 x3 x4 x5 x6 } pat).
+Tactic Notation "iPvs" open_constr(lem) constr(Hs) "as" "{"
+    simple_intropattern(x1) simple_intropattern(x2) simple_intropattern(x3)
+    simple_intropattern(x4) simple_intropattern(x5) simple_intropattern(x6)
+    simple_intropattern(x7) "}" constr(pat) :=
+  iPoseProof lem Hs as (fun H =>
+    iPvsCore H; last iDestructHyp H as { x1 x2 x3 x4 x5 x6 x7 } pat).
+Tactic Notation "iPvs" open_constr(lem) constr(Hs) "as" "{"
+    simple_intropattern(x1) simple_intropattern(x2) simple_intropattern(x3)
+    simple_intropattern(x4) simple_intropattern(x5) simple_intropattern(x6)
+    simple_intropattern(x7) simple_intropattern(x8) "}" constr(pat) :=
+  iPoseProof lem Hs as (fun H =>
+    iPvsCore H; last iDestructHyp H as { x1 x2 x3 x4 x5 x6 x7 x8 } pat).
+
+Tactic Notation "iTimeless" constr(H) :=
+  match goal with
+  | |- _ ⊢ |={_,_}=> _ =>
+     eapply tac_pvs_timeless with _ H _ _;
+       [env_cbv; reflexivity || fail "iTimeless:" H "not found"
+       |let P := match goal with |- TimelessP ?P => P end in
+        apply _ || fail "iTimeless: " P "not timeless"
+       |env_cbv; reflexivity|simpl]
+  | |- _ =>
+     eapply tac_pvs_timeless_fsa with _ _ _ _ H _ _ _;
+       [let P := match goal with |- FSASplit ?P _ _ _ _ => P end in
+        apply _ || fail "iTimeless: " P "not a pvs"
+       |env_cbv; reflexivity || fail "iTimeless:" H "not found"
+       |let P := match goal with |- TimelessP ?P => P end in
+        apply _ || fail "iTimeless: " P "not timeless"
+       |env_cbv; reflexivity|simpl]
+  end.
+
+Tactic Notation "iTimeless" constr(H) "as" constr(Hs) :=
+  iTimeless H; iDestruct H as Hs.
+
+Tactic Notation "iPvsAssert" constr(Q) "as" constr(pat) "with" constr(Hs) :=
+  let H := iFresh in
+  let Hs := spec_pat.parse_one Hs in
+  lazymatch Hs with
+  | SSplit ?lr ?Hs =>
+     eapply tac_pvs_assert with _ _ _ _ _ _ lr Hs H Q _;
+       [let P := match goal with |- FSASplit ?P _ _ _ _ => P end in
+        apply _ || fail "iPvsAssert: " P "not a pvs"
+       |env_cbv; reflexivity || fail "iPvsAssert:" Hs "not found"
+       |env_cbv; reflexivity|
+       |simpl; iDestructHyp H as pat]
+  | ?pat => fail "iPvsAssert: invalid pattern" pat
+  end.
+Tactic Notation "iPvsAssert" constr(Q) "as" constr(pat) :=
+  iPvsAssert Q as pat with "[]".
