proofmode/spec_patterns.v
@@ -1,0 +1,75 @@
+From iris.prelude Require Export strings.
+
+Inductive spec_pat :=
+  | SSplit : bool → list string → spec_pat
+  | SPersistent : spec_pat
+  | SPure : spec_pat
+  | SAlways : spec_pat
+  | SName : string → spec_pat.
+
+Module spec_pat.
+Inductive token :=
+  | TName : string → token
+  | TMinus : token
+  | TBracketL : token
+  | TBracketR : token
+  | TPersistent : token
+  | TPure : token
+  | TAlways : token.
+
+Fixpoint cons_name (kn : string) (k : list token) : list token :=
+  match kn with "" => k | _ => TName (string_rev kn) :: k end.
+Fixpoint tokenize_go (s : string) (k : list token) (kn : string) : list token :=
+  match s with
+  | "" => rev (cons_name kn k)
+  | String " " s => tokenize_go s (cons_name kn k) ""
+  | String "-" s => tokenize_go s (TMinus :: cons_name kn k) ""
+  | String "[" s => tokenize_go s (TBracketL :: cons_name kn k) ""
+  | String "]" s => tokenize_go s (TBracketR :: cons_name kn k) ""
+  | String "#" s => tokenize_go s (TPersistent :: cons_name kn k) ""
+  | String "%" s => tokenize_go s (TPure :: cons_name kn k) ""
+  | String "!" s => tokenize_go s (TAlways :: cons_name kn k) ""
+  | String a s => tokenize_go s k (String a kn)
+  end.
+Definition tokenize (s : string) : list token := tokenize_go s [] "".
+
+Fixpoint parse_go (ts : list token) (split : option (bool * list string))
+    (k : list spec_pat) : option (list spec_pat) :=
+  match split with
+  | None =>
+     match ts with
+     | [] => Some (rev k)
+     | TName s :: ts => parse_go ts None (SName s :: k)
+     | TMinus :: TBracketL :: ts => parse_go ts (Some (true,[])) k
+     | TMinus :: ts => parse_go ts None (SSplit true [] :: k)
+     | TBracketL :: ts => parse_go ts (Some (false,[])) k
+     | TAlways :: ts => parse_go ts None (SAlways :: k)
+     | TPersistent :: ts => parse_go ts None (SPersistent :: k)
+     | TPure :: ts => parse_go ts None (SPure :: k)
+     | _ => None
+     end
+  | Some (b, ss) =>
+     match ts with
+     | TName s :: ts => parse_go ts (Some (b,s :: ss)) k
+     | TBracketR :: ts => parse_go ts None (SSplit b (rev ss) :: k)
+     | _ => None
+     end
+  end.
+Definition parse (s : string) : option (list spec_pat) :=
+  parse_go (tokenize s) None [].
+
+Ltac parse s :=
+  lazymatch type of s with
+  | list spec_pat => s
+  | string => lazymatch eval vm_compute in (parse s) with
+              | Some ?pats => pats | _ => fail "invalid list spec_pat" s
+              end
+  end.
+Ltac parse_one s :=
+  lazymatch type of s with
+  | spec_pat => s
+  | string => lazymatch eval vm_compute in (parse s) with
+              | Some [?pat] => pat | _ => fail "invalid spec_pat" s
+              end
+  end.
+End spec_pat.
