proofmode/sts.v
@@ -1,0 +1,45 @@
+From iris.proofmode Require Import coq_tactics pviewshifts.
+From iris.proofmode Require Export tactics.
+From iris.program_logic Require Export sts.
+Import uPred.
+
+Section sts.
+Context `{stsG Λ Σ sts} (φ : sts.state sts → iPropG Λ Σ).
+Implicit Types P Q : iPropG Λ Σ.
+
+Lemma tac_sts_fsa {A} (fsa : FSA Λ _ A) fsaV Δ E N i γ S T Q Φ :
+  FSASplit Q E fsa fsaV Φ →
+  fsaV →
+  envs_lookup i Δ = Some (false, sts_ownS γ S T) →
+  of_envs Δ ⊢ sts_ctx γ N φ → nclose N ⊆ E →
+  (∀ s, s ∈ S → ∃ Δ',
+    envs_simple_replace i false (Esnoc Enil i (▷ φ s)) Δ = Some Δ' ∧
+    Δ' ⊢ fsa (E ∖ nclose N) (λ a, ∃ s' T',
+      ■ sts.steps (s, T) (s', T') ★ ▷ φ s' ★ (sts_own γ s' T' -★ Φ a))) →
+  Δ ⊢ Q.
+Proof.
+  intros ????? HΔ'. rewrite -(fsa_split Q); eapply (sts_fsaS φ fsa); eauto.
+  rewrite envs_lookup_sound //; simpl; apply sep_mono_r.
+  apply forall_intro=>s; apply wand_intro_l.
+  rewrite -assoc; apply const_elim_sep_l=> Hs.
+  destruct (HΔ' s) as (Δ'&?&?); clear HΔ'; auto.
+  rewrite envs_simple_replace_sound' //; simpl.
+  by rewrite right_id wand_elim_r.
+Qed.
+End sts.
+
+Tactic Notation "iSts" constr(H) "as"
+    simple_intropattern(s) simple_intropattern(Hs) :=
+  match type of H with
+  | string => eapply tac_sts_fsa with _ _ _ _ _ _ H _ _ _ _
+  | gname => eapply tac_sts_fsa with _ _ _ _ _ _ _ H _ _ _
+  | _ => fail "iSts:" H "not a string or gname"
+  end;
+    [let P := match goal with |- FSASplit ?P _ _ _ _ => P end in
+     apply _ || fail "iSts: cannot viewshift in goal" P
+    |try fast_done (* atomic *)
+    |iAssumptionCore || fail "iSts:" H "not found"
+    |iAssumption || fail "iSts: invariant not found"
+    |done || eauto with ndisj (* [eauto with ndisj] is slow *)
+    |intros s Hs; eexists; split; [env_cbv; reflexivity|simpl]].
+Tactic Notation "iSts" constr(H) "as" simple_intropattern(s) := iSts H as s ?.
