proofmode/weakestpre.v
@@ -1,0 +1,14 @@
+From iris.proofmode Require Import coq_tactics.
+From iris.proofmode Require Export pviewshifts.
+From iris.program_logic Require Export weakestpre.
+Import uPred.
+
+Section weakestpre.
+Context {Λ : language} {Σ : iFunctor}.
+Implicit Types P Q : iProp Λ Σ.
+Implicit Types Φ : val Λ → iProp Λ Σ.
+
+Global Instance fsa_split_wp E e Φ :
+  FSASplit (WP e @ E {{ Φ }})%I E (wp_fsa e) (language.atomic e) Φ.
+Proof. split. done. apply _. Qed.
+End weakestpre.
