tests/one_shot.v
@@ -1,6 +1,7 @@
 From iris.algebra Require Import one_shot dec_agree.
 From iris.program_logic Require Import hoare.
-From iris.heap_lang Require Import heap assert wp_tactics notation.
+From iris.heap_lang Require Import heap assert proofmode notation.
+From iris.proofmode Require Import invariants ghost_ownership.
 Import uPred.
 
 Definition one_shot_example : val := λ: <>,
@@ -40,96 +41,44 @@ Lemma wp_one_shot (Φ : val → iProp) :
     □ WP f2 #() {{ λ g, □ WP g #() {{ λ _, True }} }} -★ Φ (f1,f2)%V)
   ⊢ WP one_shot_example #() {{ Φ }}.
 Proof.
-  wp_let.
-  wp eapply wp_alloc; eauto with I.
-  apply forall_intro=> l; apply wand_intro_l.
-  eapply sep_elim_True_l; first by apply (own_alloc OneShotPending).
-  rewrite !pvs_frame_r; apply wp_strip_pvs.
-  rewrite !sep_exist_r; apply exist_elim=>γ.
-  (* TODO: this is horrible *)
-  trans (heap_ctx heapN ★ (|==> inv N (one_shot_inv γ l)) ★
-    (∀ f1 f2 : val,
-      (∀ n : Z, □ WP f1 #n {{ λ w, w = #true ∨ w = #false }}) ★
-      □ WP f2 #() {{ λ g, □ WP g #() {{ λ _, True }} }} -★ Φ (f1, f2)%V))%I.
-  { ecancel [heap_ctx _; ∀ _, _]%I. rewrite -inv_alloc // -later_intro.
-    apply or_intro_l'. solve_sep_entails. }
-  rewrite pvs_frame_r pvs_frame_l; apply wp_strip_pvs; wp_let.
-  rewrite -pvs_intro.
-  rewrite !assoc 2!forall_elim; eapply wand_apply_r'; first done.
-  rewrite (always_sep_dup (_ ★ _)); apply sep_mono.
-  - apply forall_intro=>n. apply: always_intro. wp_let.
-    eapply (wp_inv_timeless _ _ _ (one_shot_inv γ l)); eauto 10 with I.
-    rewrite (True_intro (inv _ _)) right_id.
-    apply wand_intro_r; rewrite sep_or_l; apply or_elim.
-    + rewrite -wp_pvs.
-      wp eapply wp_cas_suc; eauto with I ndisj.
-      rewrite (True_intro (heap_ctx _)) left_id.
-      ecancel [l ↦ _]%I; apply wand_intro_l.
-      rewrite (own_update); (* FIXME: canonical structures are not working *)
-        last by apply (one_shot_update_shoot (DecAgree n : dec_agreeR _)).
-      rewrite pvs_frame_l; apply pvs_mono, sep_intro_True_r; eauto with I.
-      rewrite /one_shot_inv -or_intro_r -(exist_intro n).
-      solve_sep_entails.
-    + rewrite sep_exist_l; apply exist_elim=>m.
-      eapply wp_cas_fail with (v':=InjRV #m) (q:=1%Qp);
-        eauto with I ndisj; strip_later.
-      ecancel [l ↦ _]%I; apply wand_intro_l, sep_intro_True_r; eauto with I.
-      rewrite /one_shot_inv -or_intro_r -(exist_intro m).
-      solve_sep_entails.
-  - apply: always_intro. wp_seq.
-    wp_focus (Load (%l))%I.
-    eapply (wp_inv_timeless _ _ _ (one_shot_inv γ l)); eauto 10 with I.
-    apply wand_intro_r.
-    trans (heap_ctx heapN ★ inv N (one_shot_inv γ l) ★ ∃ v, l ↦ v ★
-      ((v = InjLV #0 ★ own γ OneShotPending) ∨
-       ∃ n : Z, v = InjRV #n ★ own γ (Shot (DecAgree n))))%I.
-    { rewrite assoc. apply sep_mono_r, or_elim.
-      + rewrite -(exist_intro (InjLV #0)). rewrite -or_intro_l const_equiv //.
-        solve_sep_entails.
-      + apply exist_elim=> n. rewrite -(exist_intro (InjRV #n)) -(exist_intro n).
-        apply sep_mono_r, or_intro_r', sep_intro_True_l; eauto with I. }
-    rewrite !sep_exist_l; apply exist_elim=> w.
-    eapply wp_load with (q:=1%Qp) (v:=w); eauto with I ndisj.
-    rewrite -later_intro; cancel [l ↦ w]%I.
-    rewrite -later_intro; apply wand_intro_l.
-    trans (heap_ctx heapN ★ inv N (one_shot_inv γ l) ★ one_shot_inv γ l ★
-      (w = InjLV #0 ∨ (∃ n : Z, w = InjRV #n ★ own γ (Shot (DecAgree n)))))%I.
-    { cancel [heap_ctx heapN]. rewrite !sep_or_l; apply or_elim.
-      + rewrite -or_intro_l. ecancel [inv _ _]%I.
-        rewrite [(_ ★ _)%I]comm -assoc. apply const_elim_sep_l=>->.
-        rewrite const_equiv // right_id /one_shot_inv -or_intro_l .
-        solve_sep_entails.
-      + rewrite -or_intro_r !sep_exist_l; apply exist_elim=> n.
-        rewrite -(exist_intro n). ecancel [inv _ _]%I.
-        rewrite [(_ ★ _)%I]comm -assoc. apply const_elim_sep_l=>->.
-        rewrite const_equiv // left_id /one_shot_inv -or_intro_r.
-        rewrite -(exist_intro n) {1}(always_sep_dup (own _ _)).
-        solve_sep_entails. }
-    cancel [one_shot_inv γ l].
-    wp_let. rewrite -pvs_intro. apply: always_intro. wp_seq.
-    rewrite !sep_or_l; apply or_elim.
-    { rewrite assoc.
-      apply const_elim_sep_r=>->. wp_case; wp_seq; rewrite -pvs_intro; eauto with I. }
-    rewrite !sep_exist_l; apply exist_elim=> n.
-    rewrite [(w=_ ★ _)%I]comm !assoc; apply const_elim_sep_r=>->.
-    (* FIXME: why do we need to fold? *)
-    wp_case; fold of_val. wp_let. wp_focus (Load (%l))%I.
-    eapply (wp_inv_timeless _ _ _ (one_shot_inv γ l)); eauto 10 with I.
-    rewrite (True_intro (inv _ _)) right_id.
-    apply wand_intro_r; rewrite sep_or_l; apply or_elim.
-    + rewrite (True_intro (heap_ctx _)) (True_intro (l ↦ _)) !left_id.
-      rewrite -own_op own_valid_l one_shot_validI /= left_absorb.
-      apply False_elim.
-    + rewrite !sep_exist_l; apply exist_elim=> m.
-      eapply wp_load with (q:=1%Qp) (v:=InjRV #m); eauto with I ndisj; strip_later.
-      cancel [l ↦ InjRV #m]%I. apply wand_intro_r.
-      rewrite (True_intro (heap_ctx heapN)) left_id.
-      rewrite -own_op own_valid_l one_shot_validI Shot_op /= discrete_valid.
-      rewrite -assoc. apply const_elim_sep_l=> /dec_agree_op_inv [->].
-      rewrite dec_agree_idemp. apply sep_intro_True_r.
-      { rewrite /one_shot_inv -or_intro_r -(exist_intro m). solve_sep_entails. }
-      wp_case; fold of_val. wp_let. rewrite -wp_assert'.
-      wp_op; by eauto using later_intro with I.
+  iIntros "[#? Hf] /=".
+  rewrite /one_shot_example. wp_seq. wp_alloc l as "Hl". wp_let.
+  iPvs (own_alloc OneShotPending) as {γ} "Hγ"; first done.
+  iPvs (inv_alloc N _ (one_shot_inv γ l)) "[Hl Hγ]" as "#HN"; first done.
+  { iNext. iLeft. by iSplitL "Hl". }
+  iPvsIntro. iApply "Hf"; iSplit.
+  - iIntros {n} "!". wp_let.
+    iInv> N as "[[Hl Hγ]|H]"; last iDestruct "H" as {m} "[Hl Hγ]".
+    + iApply wp_pvs. wp_cas_suc. iSplitL; [|by iLeft; iPvsIntro].
+      iPvs own_update "Hγ" as "Hγ".
+      { (* FIXME: canonical structures are not working *)
+        by apply (one_shot_update_shoot (DecAgree n : dec_agreeR _)). }
+      iPvsIntro; iRight; iExists n; by iSplitL "Hl".
+    + wp_cas_fail. iSplitL. iRight; iExists m; by iSplitL "Hl". by iRight.
+  - iIntros "!". wp_seq. wp_focus (! _)%E. iInv> N as "Hγ".
+    iAssert (∃ v, l ↦ v ★ ((v = InjLV #0 ★ own γ OneShotPending) ∨
+       ∃ n : Z, v = InjRV #n ★ own γ (Shot (DecAgree n))))%I as "Hv" with "-".
+    { iDestruct "Hγ" as "[[Hl Hγ]|Hl]"; last iDestruct "Hl" as {m} "[Hl Hγ]".
+      + iExists (InjLV #0). iFrame "Hl". iLeft; by iSplit.
+      + iExists (InjRV #m). iFrame "Hl". iRight; iExists m; by iSplit. }
+    iDestruct "Hv" as {v} "[Hl Hv]". wp_load.
+    iAssert (one_shot_inv γ l ★ (v = InjLV #0 ∨ ∃ n : Z,
+      v = InjRV #n ★ own γ (Shot (DecAgree n))))%I as "[Hl #Hv]" with "-".
+    { iDestruct "Hv" as "[[% ?]|Hv]"; last iDestruct "Hv" as {m} "[% ?]"; subst.
+      + iSplit. iLeft; by iSplitL "Hl". by iLeft.
+      + iSplit. iRight; iExists m; by iSplitL "Hl". iRight; iExists m; by iSplit. }
+    iFrame "Hl". wp_let. iPvsIntro. iIntros "!". wp_seq.
+    iDestruct "Hv" as "[%|Hv]"; last iDestruct "Hv" as {m} "[% Hγ']"; subst.
+    { wp_case. wp_seq. by iPvsIntro. }
+    wp_case. wp_let. wp_focus (! _)%E.
+    iInv> N as "[[Hl Hγ]|Hinv]"; last iDestruct "Hinv" as {m'} "[Hl Hγ]".
+    { iCombine "Hγ" "Hγ'" as "Hγ". by iDestruct own_valid "Hγ" as "%". }
+    wp_load.
+    iCombine "Hγ" "Hγ'" as "Hγ".
+    iDestruct own_valid "Hγ !" as % [=->]%dec_agree_op_inv.
+    iSplitL "Hl"; [iRight; iExists m; by iSplit|].
+    wp_case. wp_let. iApply wp_assert'. wp_op=>?; simplify_eq/=.
+    iSplit. done. by iNext.
 Qed.
 
 Lemma hoare_one_shot (Φ : val → iProp) :
@@ -139,12 +88,10 @@ Lemma hoare_one_shot (Φ : val → iProp) :
       {{ True }} Snd ff #() {{ λ g, {{ True }} g #() {{ λ _, True }} }}
     }}.
 Proof.
-  apply: always_intro; rewrite left_id -wp_one_shot /=.
-  cancel [heap_ctx heapN].
-  apply forall_intro=> f1; apply forall_intro=> f2.
-  apply wand_intro_l; rewrite right_id; apply sep_mono.
-  - apply forall_mono=>n. apply always_mono; rewrite left_id. by wp_proj.
-  - apply always_mono; rewrite left_id. wp_proj.
-    apply wp_mono=> v. by apply always_mono; rewrite left_id.
+  iIntros "#? ! _". iApply wp_one_shot. iSplit; first done.
+  iIntros {f1 f2} "[#Hf1 #Hf2]"; iSplit.
+  - iIntros {n} "! _". wp_proj. iApply "Hf1" "!".
+  - iIntros "! _". wp_proj.
+    iApply wp_wand_l; iFrame "Hf2". by iIntros {v} "#? ! _".
 Qed.
 End proof.
