tests/proofmode.v
@@ -1,0 +1,42 @@
+From iris.proofmode Require Import tactics.
+
+Lemma demo_1 (M : cmraT) (P1 P2 P3 : nat → uPred M) :
+  True ⊢ (∀ (x y : nat) a b,
+    x ≡ y →
+    □ (uPred_ownM (a ⋅ b) -★
+    (∃ y1 y2 c, P1 ((x + y1) + y2) ∧ True ∧ □ uPred_ownM c) -★
+    ▷ (∀ z, P2 z) -★
+    ▷ (∀ n m : nat, P1 n → □ ((True ∧ P2 n) → □ (n = n ↔ P3 n))) -★
+    ▷ (x = 0) ∨ ∃ x z, ▷ P3 (x + z) ★ uPred_ownM b ★ uPred_ownM (core b))).
+Proof.
+  iIntros {i [|j] a b ?} "! [Ha Hb] H1 H2 H3"; setoid_subst.
+  { iLeft. by iNext. }
+  iRight.
+  iDestruct "H1" as {z1 z2 c} "(H1&_&#Hc)".
+  iRevert {a b} "Ha Hb". iIntros {b a} "Hb Ha".
+  iAssert (uPred_ownM (a ⋅ core a))%I as "[Ha #Hac]" with "[Ha]".
+  { by rewrite cmra_core_r. }
+  iFrame "Ha Hac".
+  iExists (S j + z1), z2.
+  iNext.
+  iApply "H3" { _ 0 } "H1 ! [H2] !".
+  - iSplit. done. iApply "H2".
+  - done.
+Qed.
+
+Lemma demo_2 (M : cmraT) (P1 P2 P3 P4 Q : uPred M) (P5 : nat → uPredC M):
+    (P2 ★ (P3 ★ Q) ★ True ★ P1 ★ P2 ★ (P4 ★ (∃ x:nat, P5 x ∨ P3)) ★ True)
+  ⊢ (P1 -★ (True ★ True) -★ (((P2 ∧ False ∨ P2 ∧ 0 = 0) ★ P3) ★ Q ★ P1 ★ True) ∧
+     (P2 ∨ False) ∧ (False → P5 0)).
+Proof.
+  (* Intro-patterns do something :) *)
+  iIntros "[H2 ([H3 HQ]&?&H1&H2'&foo&_)] ? [??]".
+  (* To test destruct: can also be part of the intro-pattern *)
+  iDestruct "foo" as "[_ meh]".
+  repeat iSplit; [|by iLeft|iIntros "#[]"].
+  iFrame "H2".
+  (* split takes a list of hypotheses just for the LHS *)
+  iSplitL "H3".
+  * iFrame "H3". by iRight.
+  * iSplitL "HQ". iAssumption. by iSplitL "H1".
+Qed.
